ModelCIC.v
@@ -1,8 +1,7 @@
 Require Import List Bool Models.
+Require Import ZFfunext ZFecc ZFind_nat.
+Import ZF ZFsum ZFnats ZFrelations ZFord ZFfix ZFgrothendieck.
 Require ModelZF.
-Import ZFgrothendieck.
-Import ZF ZFsum ZFnats ZFrelations ZFord ZFfix.
-Require Import ZFfunext ZFfixrec ZFecc ZFind_nat.
 
 Import ModelZF.CCM.
 Import ModelZF.BuildModel.
@@ -38,6 +37,9 @@ case_eq (nth_error e n); intros.
  rewrite H0 in H; contradiction.
 Qed.
 
+Lemma typ_kind_univ e t : typ e t kind.
+red; simpl; auto.
+Qed.
 
 (** Subtyping *)
 
@@ -106,21 +108,58 @@ apply G_cc_prod.
 Qed.
 
 
-(** Ordinals *)
+(** * Ordinals *)
 
-Definition Ord (o:set) := cst o.
+(** Closure ordinal *)
+Definition Infty := cst omega.
 
-Definition typ_ord_kind : forall e o, typ e (Ord o) kind.
+(** A special judgment (class of ordinals). It is not a set but kind does not
+    restrict to ordinals *)
+Definition typ_ord e O := forall i, val_ok e i -> isOrd (int O i).
+
+Lemma typ_ord_lift e n O :
+  typ_ord (List.skipn n e) O ->
+  typ_ord e (lift n O).
+red; intros.
+unfold lift; rewrite int_lift_rec_eq.
+rewrite V.lams0.
+apply H.
+red; intros.
+assert (nth_error e (n+n0) = value T).
+ clear H H0; revert e H1.
+ elim n; simpl; intros; trivial.
+ destruct e; auto.
+ destruct n0; discriminate H1.
+generalize (H0 _ _ H2).
+destruct T as [(T,Tm)|]; simpl; trivial.
+do 2 rewrite V.lams0.
+unfold V.shift.
+apply in_set_morph; auto with *.
+apply Tm.
+do 2 red; intros.
+simpl.
+replace (n+(S(n0+a))) with (S (n+n0+a)); auto with *.
+Qed.
+
+  Lemma typ_Infty e : typ_ord e Infty.
+red; simpl; intros; auto.
+Qed.
+
+  Lemma typ_ord_ref : forall e n T,
+    nth_error e n = value T ->
+    T <> kind ->
+    typ_ord e (lift (S n) T) ->
+    typ_ord e (Ref n).
 red; simpl; intros.
-trivial.
+generalize (H2 _ _ H); simpl.
+red in H1; specialize H1 with (1:=H2); simpl in H1.
+destruct T as [(T,Tm)|]; simpl in *.
+ eauto using isOrd_inv.
+
+ elim H0; trivial.
 Qed.
 
-Definition typ_ord_ord : forall e o o',
-  lt o o' -> typ e (Ord o) (Ord o').
-red; simpl; intros; trivial.
-Qed.
-
-
+(** Ordinal successor (also type of ordinals less or equal to the argument) *)
 Definition OSucc : term -> term.
 (*begin show*)
 intros o; left; exists (fun i => osucc (int o i)).
@@ -129,13 +168,45 @@ do 2 red; intros.
 rewrite H; reflexivity.
 Defined.
 
+Lemma typ_OSucc e O :
+  typ_ord e O ->
+  typ_ord e (OSucc O).
+red; simpl; intros.
+apply H in H0.
+auto.
+Qed.
 
+Lemma typ_ord_le e O O':
+  typ_ord e O ->
+  typ e O' (OSucc O) ->
+  typ_ord e O'.
+red; simpl; intros.
+red in H; specialize H with (1:=H1); simpl in H.
+red in H0; specialize H0 with (1:=H1); simpl in H0.
+apply isOrd_inv with (2:=H0); auto.
+Qed.
+
+Lemma typ_le_inv i e O O':
+  typ e O' (OSucc O) ->
+  val_ok e i ->
+  int O' i ⊆ int O i.
+intros.
+apply H in H0; simpl in H0.
+apply olts_le; trivial.
+Qed.
+
+(** O ≤ O *)
+Lemma typ_ord_max e O :
+  typ_ord e O ->
+  typ e O (OSucc O).
+red; simpl; intros.
+apply lt_osucc.
+apply H; trivial.
+Qed.
 
 (** Nat *)
 
 Definition Nat := cst NAT.
-
-Definition Nati (o:set) := cst (NATi o).
 
 Definition NatI : term -> term.
 (*begin show*)
@@ -147,11 +218,6 @@ apply NATi_morph.
 rewrite H; reflexivity.
 Defined.
 
-Lemma typ_nati : forall e o,
-  isOrd o -> typ e (Nati o) kind.
-red; intros; simpl; trivial.
-Qed.
-
 Lemma typ_natI : forall e o,
   typ e (NatI o) kind.
 red; intros; simpl; trivial.
@@ -161,23 +227,13 @@ Qed.
 
 Definition Zero := cst ZERO.
 
-Lemma typ_zero : forall e o,
-  isOrd o -> typ e Zero (Nati (osucc o)).
-red; simpl; intros.
-apply ZEROi_typ; trivial.
-Qed.
-
-Lemma typ_Zero : forall o e O,
-  isOrd o ->
-  typ e O (Ord o) ->
+Lemma typ_Zero : forall e O,
+  typ_ord e O ->
   typ e Zero (NatI (OSucc O)).
 red; simpl; intros.
-specialize (H0 _ H1); simpl in H0.
-assert (isOrd (int O i)).
- apply isOrd_inv with o; auto.
+apply H in H0.
 apply ZEROi_typ; trivial.
 Qed.
-
 
 (* Successor *)
 
@@ -194,35 +250,26 @@ apply inr_morph.
 apply H.
 Defined.
 
-Lemma typ_succi : forall e o i,
-  isOrd o ->
-  typ e i (Ord o) ->
-  typ e (SuccI i) (Prod (NatI i) (NatI (OSucc (lift 1 i)))). 
-intros.
-unfold SuccI.
-apply typ_abs.
- 2:discriminate.
+Lemma typ_SuccI : forall e O,
+  typ_ord e O ->
+  typ e (SuccI O) (Prod (NatI O) (NatI (OSucc (lift 1 O)))).
 red; simpl; intros.
-assert (ty_arg :=H1).
-red in ty_arg.
-specialize (ty_arg 0 _ (refl_equal _)).
-simpl in ty_arg.
-assert (isOrd (int (lift 1 i) i0)).
- specialize weakening with (1:=H0) (A:=NatI i).
- unfold Ord, lift at 2; rewrite eqterm_lift_cst; intro.
- apply H2 in H1.
- simpl in H1.
- apply isOrd_inv with o; auto.
-apply SUCCi_typ; trivial.
-apply eq_elim with (2:=ty_arg).
-fold NATi.
-apply NATi_morph.
-unfold lift; rewrite int_lift_rec_eq; reflexivity.
+apply H in H0.
+apply cc_prod_intro; intros; auto with *.
+ do 2 red; intros.
+ apply NATi_morph.
+ apply osucc_morph.
+ apply int_morph; auto with *.
+ do 2 red; intros.
+ rewrite H2; reflexivity.
+
+ unfold lift; rewrite int_lift_rec_eq.
+ rewrite V.lams0.
+ apply SUCCi_typ; auto.
 Qed.
 
-Lemma typ_SuccI : forall e o i n,
-  isOrd o ->
-  typ e i (Ord o) ->
+Lemma typ_app_SuccI : forall e i n,
+  typ_ord e i ->
   typ e n (NatI i) ->
   typ e (App (SuccI i) n) (NatI (OSucc i)). 
 intros.
@@ -230,7 +277,7 @@ apply typ_conv with (subst n (NatI (OSucc (lift 1 i)))).
 3:discriminate.
  apply typ_app with (NatI i); trivial.
  2:discriminate.
- apply typ_succi with (o:=o); trivial.
+ apply typ_SuccI; trivial.
 
  red; intros; simpl.
  unfold lift; rewrite int_lift_rec_eq.
@@ -265,14 +312,13 @@ apply NATCASE_morph_gen; intros.
  rewrite H0; rewrite H4; rewrite H2; reflexivity.
 Qed.
 
-Lemma Natcase_succ : forall o O e n fZ fS,
-  isOrd o ->
-  typ e O (Ord o) ->
+Lemma Natcase_succ : forall O e n fZ fS,
+  typ_ord e O ->
   typ e n (NatI O) ->
   eq_typ e (Natcase fZ fS (App (SuccI O) n)) (subst n fS).
 red; intros.
-red in H0; specialize H0 with (1:=H2).
-red in H1; specialize H1 with (1:=H2).
+red in H; specialize H with (1:=H1).
+red in H0; specialize H0 with (1:=H1).
 simpl in *.
 rewrite <- (fun e1 e2 => NATCASE_morph (int fZ i) (int fZ i) e1
   (fun k => int fS(V.cons k i)) (fun k => int fS(V.cons k i)) e2
@@ -281,10 +327,10 @@ rewrite <- (fun e1 e2 => NATCASE_morph (int fZ i) (int fZ i) e1
   rewrite int_subst_eq; reflexivity.
 
   intros.
-  rewrite H3; reflexivity.
+  rewrite H2; reflexivity.
 
  red; intros.
- rewrite H3; reflexivity.
+ rewrite H2; reflexivity.
 
  rewrite beta_eq; auto with *.
  red; intros.
@@ -293,47 +339,43 @@ Qed.
 
 Existing Instance NATi_morph.
 
-Lemma typ_natcase : forall o e O P fZ fS n,
-  isOrd o ->
-  typ e O (Ord o) ->
+Lemma typ_natcase : forall e O P fZ fS n,
+  typ_ord e O ->
   typ e fZ (App P Zero) ->
   typ (NatI O :: e) fS (App (lift 1 P) (App (SuccI (lift 1 O)) (Ref 0))) ->
   typ e n (NatI (OSucc O)) ->
   typ e (Natcase fZ fS n) (App P n).
 red; intros.
- red in H0; specialize H0 with (1:=H4).
- simpl in H0; red in H0.
- red in H1; specialize H1 with (1:=H4).
- simpl in H1; red in H1.
- red in H3; specialize H3 with (1:=H4).
- simpl in H3; red in H3.
- simpl; red.
- apply NATCASE_typ with (o:=int O i) (P:=fun n => app (int P i) n); trivial.
-  do 2 red; intros.
-  rewrite H5; reflexivity.
+red in H; specialize H with (1:=H3).
+simpl in H; red in H.
+red in H0; specialize H0 with (1:=H3).
+simpl in H0; red in H0.
+red in H2; specialize H2 with (1:=H3).
+simpl in H2; red in H2.
+simpl; red.
+apply NATCASE_typ with (o:=int O i) (P:=fun n => app (int P i) n); trivial.
+ do 2 red; intros.
+ rewrite H4; reflexivity.
 
-  do 2 red; intros.
-  rewrite H5; reflexivity.
+ do 2 red; intros.
+ rewrite H4; reflexivity.
 
-  apply isOrd_inv with o; trivial.
+ intros.
+ assert (val_ok (NatI O :: e) (V.cons n0 i)).
+  apply vcons_add_var; trivial.
+ apply H1 in H5; clear H1; simpl in H5.
+ change (fun k => V.cons n0 i k) with (V.cons n0 i) in H5.
+ rewrite beta_eq in H5; trivial.
+  rewrite simpl_int_lift1 in H5; trivial.
 
-  intros.
-  assert (val_ok (NatI O :: e) (V.cons n0 i)).
-   apply vcons_add_var; trivial.
-  apply H2 in H6; clear H1; simpl in H6.
-  change (fun k => V.cons n0 i k) with (V.cons n0 i) in H6.
-  rewrite beta_eq in H6; trivial.
-   rewrite simpl_int_lift1 in H6; trivial.
+  red; intros.
+  unfold SUCC; apply inr_morph; trivial.
 
-   red; intros.
-   unfold SUCC; apply inr_morph; trivial.
-
-   rewrite simpl_int_lift1; auto.
+  rewrite simpl_int_lift1; auto.
 Qed.
 
-Lemma typ_natcase' : forall o e O P fZ fS n T,
-  isOrd o ->
-  typ e O (Ord o) ->
+Lemma typ_natcase' : forall e O P fZ fS n T,
+  typ_ord e O ->
   sub_typ e (App P n) T -> 
   typ e fZ (App P Zero) ->
   typ (NatI O :: e) fS
@@ -343,15 +385,23 @@ Lemma typ_natcase' : forall o e O P fZ fS n T,
 intros.
 apply typ_subsumption with (App P n); auto.
 2:discriminate.
-apply typ_natcase with o O; trivial.
+apply typ_natcase with O; trivial.
 Qed.
 
 (********************************************************************************)
 (** Occurrences *)
 
+Module Beq.
+Definition t := bool.
+Definition eq := @eq bool.
+Definition eq_equiv : Equivalence eq := eq_equivalence.
+Existing Instance eq_equiv.
+End Beq.
+Module B := VarMap.Make(Beq).
+
 
   (* Non-occurrence : interp do not depend on variables in set [f] *)
-  Definition noccur (f:nat->bool) (T:term) : Prop :=
+  Definition noccur (f:B.map) (T:term) : Prop :=
     forall i i',
     (forall n, if f n then True else i n == i' n) ->
     int T i == int T i'.
@@ -378,18 +428,49 @@ rewrite (H0 _ _ H1).
 reflexivity.
 Qed.
 
+Lemma noc_abs a b f :
+  noccur f a ->
+  noccur (B.cons false f) b ->
+  noccur f (Abs a b).
+red; simpl; intros.
+apply cc_lam_ext.
+ apply H; trivial.
+
+ red; intros.
+ apply H0.
+ destruct n; simpl; trivial.
+ apply H1.
+Qed.
+
+Lemma noc_prod a b f :
+  noccur f a ->
+  noccur (B.cons false f) b ->
+  noccur f (Prod a b).
+red; simpl; intros.
+apply cc_prod_ext.
+ apply H; trivial.
+
+ red; intros.
+ apply H0.
+ destruct n; simpl; trivial.
+ apply H1.
+Qed.
+
+Ltac noc_tac :=
+  lazymatch goal with 
+    |- noccur _ (App _ _) => apply noc_app; noc_tac
+  | |- noccur _ (Abs _ _) => apply noc_abs; noc_tac
+  | |- noccur _ (Prod _ _) => apply noc_prod; noc_tac
+  | |- noccur _ (Ref _) => apply noc_var; reflexivity
+  | |- noccur _ _ => try (red; reflexivity) (* closed case *)
+  end.
+
 
 (********************************************************************************)
 (** Judgements with variance *)
 
-Module Beq.
-Definition t := bool.
-Definition eq := @eq bool.
-Definition eq_equiv : Equivalence eq := eq_equivalence.
-Existing Instance eq_equiv.
-End Beq.
-Module B := VarMap.Make(Beq).
 
+(** Mark stage-irrelevant functions (domain information have to be repeated) *)
 Module OTeq.
 Definition t := option term.
 Definition eq := @eq (option term).
@@ -398,7 +479,7 @@ Existing Instance eq_equiv.
 End OTeq.
 Module OT := VarMap.Make(OTeq).
 
-(* Environments with tags on ordinal and recursive function variables *)
+(** Environments with tags on ordinal and recursive function variables *)
 Record fenv := {
   tenv : env;
   ords : B.map; (* variables denoting ordinals *)
@@ -408,25 +489,33 @@ Record fenv := {
 Definition tinj e :=
   Build_fenv e (B.nil false) (OT.nil None).
 
+(** Pushing an ordinary variable *)
 Definition push_var e T :=
   Build_fenv (T::tenv e) (B.cons false (ords e)) (OT.cons None (fixs e)).
 
+(** Pushing a stage-irrelevant function *)
 Definition push_fun e dom rng :=
   Build_fenv (Prod dom rng::tenv e)
     (B.cons false (ords e)) (OT.cons (Some dom) (fixs e)).
 
+(** Pushing an ordinal (stage) variable *)
 Definition push_ord e T :=
   Build_fenv (T::tenv e) (B.cons true (ords e)) (OT.cons None (fixs e)).
 
 
-(* Additional judgments for fix body *)
+(** Semantics of contexts for variance judgments:
+    - ordinal variables follow the ordinal order
+    - stage-irrelevant function have to be compatible
+    - regular variables have to be the same
+*)
+
 Definition val_mono (e:fenv) i i' :=
     val_ok (tenv e) i /\
     val_ok (tenv e) i' /\
     forall n,
     if ords e n then i n ⊆ i' n
     else match fixs e n with
-      Some T => forall x, x ∈ int T (V.shift (S n) i) -> app (i n) x == app (i' n) x
+      Some T => fcompat (int T (V.shift (S n) i)) (i n) (i' n)
     | _ => i n == i' n
     end.
 
@@ -436,6 +525,7 @@ split;[idtac|split]; simpl; auto with *.
 intro n.
 destruct (ords e n); auto with *.
 destruct (fixs e n); auto with *.
+red; auto with *.
 Qed.
 
 Lemma val_push_var : forall e i i' x x' T,
@@ -492,27 +582,29 @@ destruct 1 as (?&?&?); split;[idtac|split]; trivial.
  destruct (ords e n); trivial.
 Qed.
 
+(** Invariance judgement *)
+Definition var_equals e M :=
+  forall i i', val_mono e i i' -> int M i == int M i'.
+
 (** Function Extension judgment *)
-Definition fx_extends e dom M :=
+Definition var_compat e dom M :=
   forall i i', val_mono e i i' ->
   fcompat (int dom i) (int M i) (int M i').
 
 (** Covariance judgment *)
-Definition fx_sub e M :=
+Definition var_mono e M :=
   forall i i', val_mono e i i' ->
   int M i ⊆ int M i'.
 
-(** Invariance *)
-Definition fx_equals e M :=
-  forall i i', val_mono e i i' -> int M i == int M i'.
 
-Definition spec_var e n :=
-  ords e n || match fixs e n with Some _ => true | _ => false end.
+(** Invariance rules *)
+  Definition spec_var e n :=
+    ords e n || match fixs e n with Some _ => true | _ => false end.
 
-  Lemma fx_eq_noc : forall e t,
+  Lemma var_eq_noc : forall e t,
     noccur (spec_var e) t ->
-    fx_equals e t.
-unfold noccur, fx_equals, spec_var; intros.
+    var_equals e t.
+unfold noccur, var_equals, spec_var; intros.
 apply H; intros.
 destruct H0 as (_,(_,H0)).
 generalize (H0 n).
@@ -520,22 +612,22 @@ destruct (ords e n); simpl; trivial.
 destruct (fixs e n); simpl; trivial.
 Qed.
 
-  Lemma fx_eq_app : forall e u v,
-    fx_equals e u ->
-    fx_equals e v ->
-    fx_equals e (App u v).
-unfold fx_equals; intros.
+  Lemma var_eq_app : forall e u v,
+    var_equals e u ->
+    var_equals e v ->
+    var_equals e (App u v).
+unfold var_equals; intros.
 specialize H with (1:=H1).
 specialize H0 with (1:=H1).
 simpl.
 rewrite H; rewrite H0; reflexivity.
 Qed.
 
-  Lemma fx_eq_abs : forall e T M,
-    fx_equals e T ->
-    fx_equals (push_var e T) M ->
-    fx_equals e (Abs T M).
-unfold fx_equals; intros.
+  Lemma var_eq_abs : forall e T M,
+    var_equals e T ->
+    var_equals (push_var e T) M ->
+    var_equals e (Abs T M).
+unfold var_equals; intros.
 simpl.
 apply lam_ext; auto.
 red; intros.
@@ -547,106 +639,88 @@ apply val_push_var; auto.
  rewrite <- H3; rewrite <- H; trivial.
 Qed.
 
-  Lemma fx_eq_rec_call : forall e n x T U,
+  Lemma var_eq_prod : forall e T U,
+    var_equals e T ->
+    var_equals (push_var e T) U ->
+    var_equals e (Prod T U).
+red; simpl; intros.
+specialize (H _ _ H1).
+apply cc_prod_ext; trivial.
+red; intros.
+apply H0.
+apply val_push_var; auto with *.
+change (el T i' x').
+rewrite <- H3.
+apply in_int_el.
+rewrite <- H; trivial.
+Qed.
+
+  Lemma var_eq_OSucc : forall e O,
+    var_equals e O ->
+    var_equals e (OSucc O).
+unfold var_equals; simpl; intros.
+apply osucc_morph; apply H; trivial.
+Qed.
+
+  Lemma var_eq_Natcase : forall e O f1 f2 c,
+    typ_ord (tenv e) O ->
+    var_mono e O ->
+    var_equals e f1 ->
+    var_equals (push_var e (NatI O)) f2 ->
+    typ (tenv e) c (NatI (OSucc O)) ->
+    var_equals e c ->
+    var_equals e (Natcase f1 f2 c).
+red; intros e O f1 f2 c tyO H0 H1 H2 tyc H3 i i' H4.
+simpl.
+change (fun k => i k) with i.
+change (fun k => i' k) with i'.
+assert (ord : isOrd (int O i)).
+ apply (tyO _ (proj1 H4)).
+assert (ord' : isOrd (int O i')).
+ apply (tyO _ (proj1 (proj2 H4))).
+assert (int c i ∈ NATi (osucc (int O i))).
+ destruct H4 as (H4,_).
+ apply tyc in H4; trivial.
+apply NATCASE_morph_gen; intros; auto.
+ apply H3; trivial.
+
+ apply H1; trivial.
+
+ apply H2.
+ red in H0; specialize H0 with (1:=H4).
+ rewrite H5 in H.
+ apply SUCCi_inv_typ in H; auto.
+ apply val_push_var; simpl; auto.
+ rewrite <- H6.
+ clear H5 H6 x'; revert x H.
+ apply TI_mono; auto.
+Qed.
+
+(** Stage-irrelevance rules *)
+  Lemma var_comp_ref : forall e dom n T,
     ords e n = false ->
     fixs e n = Some T ->
     T <> kind ->
-    typ (tenv e) (Ref n) (Prod (lift (S n) T) U) ->
-    fx_equals e x ->
-    typ (tenv e) x (lift (S n) T) ->
-    fx_equals e (App (Ref n) x).
-unfold fx_equals; intros.
-simpl.
-specialize H3 with (1:=H5).
-rewrite <- H3.
-destruct H5 as (Hty,(Hty',Hrec)).
-specialize Hrec with n.
-rewrite H in Hrec; rewrite H0 in Hrec.
-apply Hrec.
-red in H4; specialize H4 with (1:=Hty); trivial.
-destruct T as [(T,Tm)|]; simpl in H4|-*; auto.
- rewrite V.lams0 in H4; assumption.
-
- elim H1; trivial.
+    eq_typ (tenv e) (lift (S n) T) dom ->
+    var_compat e dom (Ref n).
+unfold var_compat; simpl; intros.
+destruct H3 as (Hty,(Hty',Hrec)).
+generalize (Hrec n).
+rewrite H; rewrite H0.
+unfold fcompat; intros.
+apply H3.
+revert H4.
+rewrite <- (H2 _ Hty).
+unfold lift; rewrite int_lift_rec_eq.
+rewrite V.lams0; trivial.
 Qed.
-
-  (* Covariance *)
-
-  Lemma fx_equals_sub : forall e M, fx_equals e M -> fx_sub e M.
-unfold fx_sub, fx_equals; intros.
-apply H in H0.
-rewrite H0; reflexivity.
-Qed.
-
-  Lemma var_sub : forall e n,
-    ords e n = true ->
-    fx_sub e (Ref n).
-unfold fx_sub; intros.
-destruct H0 as (_,(_,H0)).
-generalize (H0 n); rewrite H.
-simpl; trivial.
-Qed.
-
-Lemma fx_sub_prod : forall e T U,
-  fx_equals e T ->
-  fx_sub (push_var e T) U ->
-  fx_sub e (Prod T U).
-red; simpl; intros.
-specialize (H _ _ H1).
-apply cc_prod_covariant; intros; auto.
- red; red; intros.
- rewrite H3; reflexivity.
-
- apply H0.
- apply val_push_var; auto with *.
-  change (el T i' x).
-  apply in_int_el.
-  rewrite <- H; trivial.
-Qed.
-
-  Lemma NATi_sub : forall e o O,
-    isOrd o ->
-    typ (tenv e) O (Ord o) ->
-    fx_sub e O ->
-    fx_sub e (NatI O).
-unfold fx_sub; intros.
-simpl.
-apply TI_mono; auto.
- destruct H2 as (_,(H2,_)).
- apply H0 in H2.
- apply isOrd_inv with o; auto.
-
- destruct H2 as (H2,_).
- apply H0 in H2.
- apply isOrd_inv with o; auto.
-Qed.
-
-  Lemma OSucc_sub : forall e O,
-    fx_sub e O ->
-    fx_sub e (OSucc O).
-unfold fx_sub; simpl; intros.
-red; intros.
-unfold osucc in *.
-apply subset_intro.
- apply power_intro; intros.
- apply H with (1:=H0); trivial.
- apply power_elim with z; trivial.
- apply subset_elim1 in H1; trivial.
-
- apply subset_elim2 in H1.
- destruct H1.
- rewrite H1; trivial.
-Qed.
-
-  (* Function subtyping *)
-
-  Lemma fx_abs : forall e U T M,
-    fx_sub e T ->
-    fx_equals (push_var e T) M ->
+  Lemma abs_compat : forall e U T M,
+    var_mono e T ->
+    var_equals (push_var e T) M ->
     typ (T::tenv e) M U ->
     U <> kind ->
-    fx_extends e T (Abs T M).
-unfold fx_sub, fx_equals, fx_extends; intros.
+    var_compat e T (Abs T M).
+unfold var_mono, var_equals, var_compat; intros.
 specialize H with (1:=H3).
 simpl.
 red; intros.
@@ -665,42 +739,106 @@ fold app.
  rewrite H6; reflexivity.
 Qed.
 
-
-Lemma Natcase_fx_eq : forall o e O f1 f2 c,
-  isOrd o ->
-  typ (tenv e) O (Ord o) ->
-  fx_sub e O ->
-  fx_equals e f1 ->
-  fx_equals (push_var e (NatI O)) f2 ->
-  typ (tenv e) c (NatI (OSucc O)) ->
-  fx_equals e c ->
-  fx_equals e (Natcase f1 f2 c).
-red; intros o e O f1 f2 c H tyO H0 H1 H2 tyc H3 i i' H4.
-simpl.
-assert (ord : isOrd (int O i)).
- destruct H4 as (H4,_); apply tyO in H4.
- apply isOrd_inv with o; trivial.
-assert (ord' : isOrd (int O i')).
- destruct H4 as (_,(H4,_)); apply tyO in H4.
- apply isOrd_inv with o; trivial.
-assert (int c i ∈ NATi (osucc (int O i))).
- destruct H4 as (H4,_).
- apply tyc in H4; trivial.
-apply NATCASE_morph_gen; intros; auto.
- apply H3; trivial.
-
- apply H1; trivial.
-
- apply H2.
- red in H0; specialize H0 with (1:=H4).
- rewrite H6 in H5.
- apply SUCCi_inv_typ in H5; auto.
- apply val_push_var; simpl; auto.
- rewrite <- H7.
- clear H6 H7 x'; revert x H5.
- apply TI_mono; auto.
+  Lemma succ_compat e O :
+    typ_ord (tenv e) O ->
+    var_mono e O ->
+    var_compat e (NatI O) (SuccI O).
+do 2 red; simpl; intros.
+red in H, H0.
+specialize H0 with (1:=H1).
+rewrite cc_beta_eq; auto with *.
+rewrite cc_beta_eq; auto with *.
+revert H2; apply TI_mono; auto with *.
+ apply H; apply H1.
+ apply H; apply H1.
 Qed.
 
+
+  Lemma var_comp_app : forall e dom u v,
+    dom <> kind ->
+    var_compat e dom u ->
+    typ (tenv e) v dom ->
+    var_equals e v ->
+    var_equals e (App u v).
+unfold var_equals; intros.
+simpl.
+transitivity (app (int u i') (int v i)).
+ do 2 red in H0.
+ apply H0; trivial.
+ red in H1.
+ specialize H1 with (1:=proj1 H3).
+ revert H1; destruct dom; trivial.
+ elim H; trivial.
+
+ rewrite <- H2 with (1:=H3).
+ reflexivity.
+Qed.
+
+
+(** Covariance rules *)
+
+  Lemma var_eq_sub : forall e M, var_equals e M -> var_mono e M.
+unfold var_mono, var_equals; intros.
+apply H in H0.
+rewrite H0; reflexivity.
+Qed.
+
+  Lemma var_mono_ref : forall e n,
+    ords e n = true ->
+    var_mono e (Ref n).
+unfold var_mono; intros.
+destruct H0 as (_,(_,H0)).
+generalize (H0 n); rewrite H.
+simpl; trivial.
+Qed.
+
+  Lemma var_mono_prod : forall e T U,
+    var_equals e T ->
+    var_mono (push_var e T) U ->
+    var_mono e (Prod T U).
+red; simpl; intros.
+specialize (H _ _ H1).
+apply cc_prod_covariant; intros; auto.
+ red; red; intros.
+ rewrite H3; reflexivity.
+
+ apply H0.
+ apply val_push_var; auto with *.
+  change (el T i' x).
+  apply in_int_el.
+  rewrite <- H; trivial.
+Qed.
+
+  Lemma var_mono_NATi : forall e O,
+    typ_ord (tenv e) O ->
+    var_mono e O ->
+    var_mono e (NatI O).
+unfold var_mono; intros.
+simpl.
+assert (oo : isOrd (int O i)).
+ apply (H _ (proj1 H1)).
+assert (oo' : isOrd (int O i')).
+ apply (H _ (proj1 (proj2 H1))).
+clear H.
+apply TI_mono; auto.
+Qed.
+
+  Lemma var_mono_OSucc : forall e O,
+    var_mono e O ->
+    var_mono e (OSucc O).
+unfold var_mono; simpl; intros.
+red; intros.
+unfold osucc in *.
+apply subset_intro.
+ apply power_intro; intros.
+ apply H with (1:=H0); trivial.
+ apply power_elim with z; trivial.
+ apply subset_elim1 in H1; trivial.
+
+ apply subset_elim2 in H1.
+ destruct H1.
+ rewrite H1; trivial.
+Qed.
 
 
 (*****************************************************************************)
@@ -727,18 +865,16 @@ Defined.
 
 Section NatFixRules.
 
-  Variable infty : set.
-  Hypothesis infty_ord : isOrd infty.
   Variable E : fenv.
   Let e := tenv E.
   Variable O U M : term.
   Hypothesis M_nk : ~ eq_term M kind.
-  Hypothesis ty_O : typ e O (Ord infty).
+  Hypothesis ty_O : typ_ord e O.
   Hypothesis ty_M : typ (Prod (NatI (Ref 0)) U::OSucc O::e)
     M (Prod (NatI (OSucc (Ref 1)))
          (lift1 1 (subst_rec (OSucc (Ref 0)) 1 (lift_rec 1 2 U)))).
 
-  Hypothesis stab : fx_extends
+  Hypothesis stab : var_compat
     (push_fun (push_ord E (OSucc O)) (NatI (Ref 0)) U)
     (NatI (OSucc (Ref 1)))
     M.
@@ -756,20 +892,20 @@ do 2 red; intros.
 rewrite H0;reflexivity.
 Qed.
 
-  Hypothesis fx_sub_U :
-    fx_sub (push_var (push_ord E (OSucc O)) (NatI (OSucc (Ref 0)))) U.
+  Hypothesis var_mono_U :
+    var_mono (push_var (push_ord E (OSucc O)) (NatI (OSucc (Ref 0)))) U.
 
 
   Lemma ty_fix_body : forall i o f,
-   val_ok e i ->
-   lt o (osucc (int O i)) ->
-   f ∈ prod (NATi o) (fun x => int U (V.cons x (V.cons o i))) ->
-   F i o f ∈
-   prod (NATi (osucc o)) (fun x => int U (V.cons x (V.cons (osucc o) i))).
+    val_ok e i ->
+    o < osucc (int O i) ->
+    f ∈ prod (NATi o) (fun x => int U (V.cons x (V.cons o i))) ->
+    F i o f ∈
+    prod (NATi (osucc o)) (fun x => int U (V.cons x (V.cons (osucc o) i))).
 unfold F; intros.
 specialize (ty_O _ H); simpl in ty_O.
 assert (isOrd (int O i)).
- apply isOrd_inv with infty; trivial.
+ auto.
 refine (eq_elim _ _ _ _ (ty_M (V.cons f (V.cons o i)) _)); simpl.
  apply prod_ext; auto with *.
  red; intros.
@@ -804,8 +940,7 @@ Qed.
     NAT_ord_irrel (int O i) (F i) (fun o' x => int U (V.cons x (V.cons o' i))).
 red; red; intros.
 assert (isOrd (int O i)).
- apply ty_O in H.
- apply isOrd_inv with infty; auto.
+ auto.
 red in stab.
 assert (Hstab := stab (V.cons f (V.cons o i)) (V.cons g (V.cons o' i))).
 simpl in Hstab.
@@ -829,7 +964,7 @@ Qed.
    x == x' ->
    int U (V.cons x (V.cons o i)) ⊆ int U (V.cons x' (V.cons o' i)).
 intros.
-apply fx_sub_U.
+apply var_mono_U.
 apply val_push_var; simpl; auto.
  apply val_push_ord; simpl; auto; change (int O (fun k => i k)) with (int O i).
   apply val_mono_refl; trivial.
@@ -848,16 +983,14 @@ Qed.
 
   Hint Resolve morph_fix_body ext_fun_ty ty_fix_body fix_codom_mono fix_body_irrel.
 
-Lemma nat_fix_eqn : forall i,
-  val_ok e i ->
-  NATREC (F i) (int O i) ==
-  cc_lam (NATi (int O i))
-    (fun x => cc_app (F i (int O i) (NATREC (F i) (int O i))) x).
+  Lemma nat_fix_eqn : forall i,
+    val_ok e i ->
+    NATREC (F i) (int O i) ==
+    cc_lam (NATi (int O i))
+      (fun x => cc_app (F i (int O i) (NATREC (F i) (int O i))) x).
 intros.
 assert (oi : isOrd (int O i)).
- apply ty_O in H.
- simpl in H.
- apply isOrd_inv with infty; trivial.
+ auto.
 apply NATREC_eqn with
   (ord:=int O i)
   (U:=fun o x => int U (V.cons x (V.cons o i))); auto.
@@ -867,14 +1000,11 @@ apply ole_lts; auto.
 Qed.
 
 
-Lemma typ_nat_fix :
-  typ e (NatFix O M) (Prod (NatI O) (subst_rec O 1 U)).
+  Lemma typ_nat_fix : typ e (NatFix O M) (Prod (NatI O) (subst_rec O 1 U)).
 red; intros.
 simpl.
 assert (isOrd (int O i)).
- apply ty_O in H.
- simpl in H.
- apply isOrd_inv with infty; trivial.
+ auto.
 apply eq_elim with
    (prod (NATi (int O i)) (fun x => int U (V.cons x (V.cons (int O i) i)))).
  apply prod_ext.
@@ -896,10 +1026,10 @@ apply ole_lts; trivial.
 Qed.
 
 
-Lemma nat_fix_eq : forall N,
-  typ e N (NatI O) ->
-  eq_typ e (App (NatFix O M) N)
-           (App (subst O (subst (lift 1 (NatFix O M)) M)) N).
+  Lemma nat_fix_eq : forall N,
+    typ e N (NatI O) ->
+    eq_typ e (App (NatFix O M) N)
+             (App (subst O (subst (lift 1 (NatFix O M)) M)) N).
 red; intros.
 change
  (app (NATREC (F i) (int O i)) (int N i) ==
@@ -911,31 +1041,27 @@ simpl.
 change (int O (fun k => i k)) with (int O i).
 assert (O_lt := @ty_O _ H0).
 simpl in O_lt.
-assert (isOrd (int O i)).
- apply isOrd_inv with infty; trivial.
 rewrite nat_fix_eqn; trivial.
 rewrite beta_eq.
  reflexivity.
 
  red; intros.
- rewrite H3; reflexivity.
+ rewrite H2; reflexivity.
 
  apply H; trivial.
 Qed.
 
-Lemma nat_fix_extend :
-  fx_sub E O ->
-  fx_extends E (NatI O) (NatFix O M).
+  Lemma var_comp_fix :
+    var_mono E O ->
+    var_compat E (NatI O) (NatFix O M).
 intro subO.
 do 2 red; intros.
 assert (isval := proj1 H).
 assert (isval' := proj1 (proj2 H)).
 assert (oo: isOrd (int O i)).
- apply isOrd_inv with infty; trivial.
- apply ty_O; trivial.
+ auto.
 assert (oo': isOrd (int O i')).
- apply isOrd_inv with infty; trivial.
- apply ty_O; trivial.
+ auto.
 assert (inclo: int O i ⊆ int O i').
  apply subO in H; trivial.
 clear subO.
@@ -1048,9 +1174,9 @@ rewrite cc_beta_eq; auto with *.
  do 2 red; intros; apply cc_app_morph; auto with *.
 Qed.
 
-Lemma nat_fix_equals :
-  fx_equals E O ->
-  fx_equals E (NatFix O M).
+  Lemma var_eq_fix :
+    var_equals E O ->
+    var_equals E (NatFix O M).
 red; intros.
 assert (ty1 := typ_nat_fix _ (proj1 H0)); simpl in ty1.
 assert (ty2 := typ_nat_fix _ (proj1 (proj2 H0))); simpl in ty2.
@@ -1063,46 +1189,27 @@ apply cc_lam_ext; auto with *.
 
  red; intros.
  rewrite <- H2.
- apply nat_fix_extend; trivial.
- apply fx_equals_sub; trivial.
+ apply var_comp_fix; trivial.
+ apply var_eq_sub; trivial.
 Qed.
 
 End NatFixRules.
 
 Print Assumptions typ_nat_fix.
 
-
-Lemma typ_nat_fix' : forall infty e O U M T,
-       isOrd infty ->
-       typ e O (Ord infty) ->
-       typ (Prod (NatI (Ref 0)) U :: OSucc O :: e) M
-         (Prod (NatI (OSucc (Ref 1)))
-           (lift1 1 (subst_rec (OSucc (Ref 0)) 1 (lift_rec 1 2 U)))) ->
-       fx_extends (push_fun (push_ord (tinj e) (OSucc O)) (NatI (Ref 0)) U)
-         (NatI (OSucc (Ref 1))) M ->
-       fx_sub (push_var (push_ord (tinj e) (OSucc O)) (NatI (OSucc (Ref 0)))) U ->
-       sub_typ e (Prod (NatI O) (subst_rec O 1 U)) T ->
-       typ e (NatFix O M) T.
-intros.
-apply typ_subsumption with (Prod (NatI O) (subst_rec O 1 U)); auto.
-2:discriminate.
-change e with (tenv (tinj e)).
-apply typ_nat_fix with (infty:=infty); trivial.
-Qed.
-
 (****************************************************************************************)
 (** Compound judgements : typing + variance *)
 
+Definition typ_inv e M T :=
+  var_equals e M /\ typ (tenv e) M T.
+
 Definition typ_ext e M A B :=
-  fx_extends e A M /\ typ (tenv e) M (Prod A B).
+  var_compat e A M /\ typ (tenv e) M (Prod A B).
 
 Definition typ_mono e M T :=
-  fx_sub e M /\ typ (tenv e) M T.
+  var_mono e M /\ typ (tenv e) M T.
 
-Definition typ_impl e M T :=
-  fx_equals e M /\ typ (tenv e) M T.
-
-Instance typ_impl_morph e : Proper (eq_term ==> eq_term ==> iff) (typ_impl e).
+Instance typ_inv_morph e : Proper (eq_term ==> eq_term ==> iff) (typ_inv e).
 apply morph_impl_iff2; auto with *.
 do 4 red; intros.
 destruct H1; split.
@@ -1112,15 +1219,235 @@ destruct H1; split.
  rewrite <- H; rewrite <- H0; auto.
 Qed.
 
-Lemma typ_var_impl : forall e n t T,
+
+(** Inclusion relation between judgements *)
+  Lemma typ_inv_mono : forall e M T, typ_inv e M T -> typ_mono e M T.
+destruct 1; split; trivial.
+apply var_eq_sub; trivial.
+Qed.
+
+  Lemma typ_inv_ext : forall e M A B, typ_inv e M (Prod A B) -> typ_ext e M A B.
+destruct 1; split; trivial.
+do 2 red; intros.
+apply H in H1.
+rewrite H1; reflexivity.
+Qed.
+
+(** Inference rules *)
+  Lemma typ_inv_subsumption e M T T' :
+    typ_inv e M T -> sub_typ (tenv e) T T' -> T <> kind -> typ_inv e M T'.
+destruct 1; split; trivial.
+apply typ_subsumption with (2:=H1); trivial.
+Qed.
+
+(** Typing the three kind of variables *)
+  Lemma typ_inv_ref : forall e n T,
+    spec_var e n = false ->
+    nth_error (tenv e) n = value T ->
+    typ_inv e (Ref n) (lift (S n) T).
+intros.
+split.
+ apply var_eq_noc; apply noc_var; trivial.
+ apply typ_var; trivial.
+Qed.
+
+
+(* Not really useful since (Ref n) should be an ordinal... *)
+  Lemma typ_mono_ref : forall e n T,
+    ords e n = true ->
+    nth_error (tenv e) n = value T ->
+    typ_mono e (Ref n) (lift (S n) T).
+split.
+ apply var_mono_ref; trivial.
+ apply typ_var; trivial.
+Qed.
+
+ Lemma typ_ext_ref e n A B :
+    ords e n = false ->
+    fixs e n = Some A ->
+    A <> kind ->
+    nth_error (tenv e) n = value (Prod A B) ->
+    typ_ext e (Ref n) (lift (S n) A) (lift1 (S n) B).
+split.
+ apply var_comp_ref with (2:=H0); trivial.
+ reflexivity.
+
+ eapply typ_conv.
+  apply typ_var with (1:=H2).
+  2:discriminate.
+
+  unfold lift; rewrite eq_lift_prod; reflexivity.
+Qed.
+
+(** Abstraction *)
+  Lemma typ_inv_abs : forall e U T M,
+    U <> kind ->
+    var_equals e T ->
+    typ_inv (push_var e T) M U ->
+    typ_inv e (Abs T M) (Prod T U).
+destruct 3; split.
+ apply var_eq_abs; trivial.
+
+ apply typ_abs; trivial.
+Qed.
+
+  Lemma typ_ext_abs : forall e U T M,
+    var_mono e T ->
+    typ_inv (push_var e T) M U ->
+    U <> kind ->
+    typ_ext e (Abs T M) T U.
+destruct 2; split.
+ apply abs_compat with U; trivial.
+
+ apply typ_abs; trivial.
+Qed.
+
+(** Application *)
+
+  Lemma typ_ext_app : forall e u v A B,
+    A <> kind ->
+    typ_ext e u A B -> 
+    typ_inv e v A ->
+    typ_inv e (App u v) (subst v B).
+intros.
+destruct H0; destruct H1; split.
+ apply var_comp_app with (2:=H0); trivial.
+
+ apply typ_app with A; trivial.
+Qed.
+
+(** Natural numbers: type and constructors *)
+
+(*
+  Lemma mono_NATi : forall e O,
+    typ_mono e O Ord ->
+    var_mono e (NatI O).
+destruct 1.
+apply var_mono_NATi; auto.
+Qed.
+*)
+(*
+  Lemma mono_OSucc : forall e O o,
+    isOrd o ->
+    typ_mono e O O' ->
+    typ_mono e (OSucc O) (OSucc O').
+destruct 2.
+split.
+ apply var_mono_OSucc; trivial.
+
+ red; simpl; intros.
+ apply lt_osucc_compat; trivial.
+ apply H1; trivial.
+Qed.
+*)
+
+  Lemma typ_inv_Zero e O :
+    typ_ord (tenv e) O ->
+(*    var_mono e O -> *)
+    typ_inv e Zero (NatI (OSucc O)).
+split; simpl.
+ red; reflexivity.
+ apply typ_Zero; trivial.
+Qed.
+
+
+  Lemma typ_inv_Succ e O :
+    typ_ord (tenv e) O ->
+    var_equals e O ->
+    typ_inv e (SuccI O) (Prod (NatI O) (NatI (OSucc (lift 1 O)))).
+split; simpl.
+ red; simpl; intros.
+ apply cc_lam_ext.
+  apply NATi_morph.
+  apply H0; trivial.
+
+  red; intros. 
+  rewrite H3; reflexivity.
+
+ apply typ_SuccI; trivial.
+Qed.
+
+  Lemma typ_ext_Succ e O :
+    typ_ord (tenv e) O ->
+    var_mono e O ->
+    typ_ext e (SuccI O) (NatI O) (NatI (OSucc (lift 1 O))).
+split; simpl.
+ do 2 red; simpl; intros.
+ rewrite cc_beta_eq; auto with *.
+ rewrite cc_beta_eq; auto with *.
+ change (x ∈ NATi (int O i')).
+ revert H2; apply TI_mono; auto with *.
+  apply H; apply H1.
+  apply H; apply H1.
+
+ apply typ_SuccI; trivial.
+Qed.
+
+
+(** Case-analysis *)
+  Lemma typ_inv_natcase : forall e O P fZ fS n T,
+    typ_ord (tenv e) O ->
+    var_mono e O ->
+    sub_typ (tenv e) (App P n) T -> 
+    typ_inv e fZ (App P Zero) ->
+    typ_inv (push_var e (NatI O)) fS
+      (App (lift 1 P) (App (SuccI (lift 1 O)) (Ref 0))) ->
+    typ_inv e n (NatI (OSucc O)) ->
+    typ_inv e (Natcase fZ fS n) T.
+intros.
+destruct H2.
+destruct H3.
+simpl in H6.
+destruct H4.
+split.
+ apply var_eq_Natcase with O; trivial.
+
+ apply typ_natcase' with O P; trivial.
+Qed.
+
+(** Fixpoint *)
+
+  Lemma typ_ext_fix : forall e O U M,
+    typ_ord (tenv e) O ->
+    var_mono e O ->
+    typ_ext (push_fun (push_ord e (OSucc O)) (NatI (Ref 0)) U) M
+      (NatI (OSucc (Ref 1))) (lift1 1 (subst_rec (OSucc (Ref 0)) 1 (lift_rec 1 2 U))) ->
+    var_mono (push_var (push_ord e (OSucc O)) (NatI (OSucc (Ref 0)))) U ->
+    typ_ext e (NatFix O M) (NatI O) (subst_rec O 1 U).
+intros e O U M tyO inclO (extM,tyM) tyU.
+split.
+ apply var_comp_fix with U; trivial.
+
+ apply typ_nat_fix; trivial.
+Qed.
+
+  Lemma typ_inv_fix : forall e O U M,
+    typ_ord (tenv e) O ->
+    var_equals e O ->
+    typ_ext (push_fun (push_ord e (OSucc O)) (NatI (Ref 0)) U) M
+      (NatI (OSucc (Ref 1))) (lift1 1 (subst_rec (OSucc (Ref 0)) 1 (lift_rec 1 2 U))) ->
+    var_mono (push_var (push_ord e (OSucc O)) (NatI (OSucc (Ref 0)))) U ->
+    typ_inv e (NatFix O M) (Prod (NatI O) (subst_rec O 1 U)).
+intros e O U M tyO inclO (extM,tyM) tyU.
+split.
+ apply var_eq_fix with U; trivial.
+
+ apply typ_nat_fix; trivial.
+Qed.
+
+
+
+(** Derived rules for practical examples (basically applies subsumption beforehand) *)
+
+  Lemma typ_inv_ref' : forall e n t T,
     spec_var e n = false ->
     nth_error (tenv e) n = value t ->
     t <> kind ->
     sub_typ (tenv e) (lift (S n) t) T ->
-    typ_impl e (Ref n) T.
+    typ_inv e (Ref n) T.
 intros.
 split.
- apply fx_eq_noc; apply noc_var; trivial.
+ apply var_eq_noc; apply noc_var; trivial.
 
  apply typ_subsumption with (lift (S n) t); trivial.
   apply typ_var; trivial.
@@ -1129,36 +1456,18 @@ split.
   discriminate.
 Qed.
 
-  Lemma impl_abs : forall e U T T' M,
-    U <> kind ->
-    eq_typ (tenv e) T T' ->
-    fx_equals e T ->
-    typ_impl (push_var e T) M U ->
-    typ_impl e (Abs T M) (Prod T' U).
-destruct 4; split.
- apply fx_eq_abs; trivial.
-
- apply typ_conv with (Prod T U); auto.
-  apply typ_abs; trivial.
-
-  apply eq_typ_prod; trivial.
-  reflexivity.
-
-  discriminate.
-Qed.
-
-Lemma impl_app : forall e u v V Ur T,
-  V <> kind ->
-  Ur <> kind ->
-  sub_typ (tenv e) (subst v Ur) T ->
-  typ_impl e u (Prod V Ur) ->
-  typ_impl e v V ->
-  typ_impl e (App u v) T.
+  Lemma typ_inv_app : forall e u v V Ur T,
+    V <> kind ->
+    Ur <> kind ->
+    sub_typ (tenv e) (subst v Ur) T ->
+    typ_inv e u (Prod V Ur) ->
+    typ_inv e v V ->
+    typ_inv e (App u v) T.
 intros.
 destruct H2.
 destruct H3.
 split.
- apply fx_eq_app; trivial.
+ apply var_eq_app; trivial.
 
  apply typ_subsumption with (subst v Ur); trivial.
   apply typ_app with V; auto.
@@ -1167,154 +1476,23 @@ split.
   discriminate.
 Qed.
 
-  Lemma NATi_fx_sub : forall e o O,
-    isOrd o ->
-    typ_mono e O (Ord o) ->
-    fx_sub e (NatI O).
-destruct 2.
-apply NATi_sub with (o:=o); trivial.
-Qed.
-
-  Lemma OSucc_fx_sub : forall e O o,
-    isOrd o ->
-    typ_mono e O (Ord o)->
-    typ_mono e (OSucc O) (Ord (osucc o)).
-destruct 2.
-split.
- apply OSucc_sub; trivial.
-
- red; simpl; intros.
- apply lt_osucc_compat; trivial.
- apply H1; trivial.
-Qed.
-
-  Lemma typ_var_mono : forall e n t T,
-    ords e n = true ->
-    nth_error (tenv e) n = value t ->
-    t <> kind ->
-    sub_typ (tenv e) (lift (S n) t) T ->
-    typ_mono e (Ref n) T.
-intros.
-split.
- apply var_sub; trivial.
-
- apply typ_subsumption with (lift (S n) t); trivial.
-  apply typ_var; trivial.
-
-  destruct t as [(t,tm)|]; simpl in *; auto.
-  discriminate.
-Qed.
-
-  Lemma ext_abs : forall e U T M,
-    fx_sub e T ->
-    typ_impl (push_var e T) M U ->
-    U <> kind ->
-    typ_ext e (Abs T M) T U.
-destruct 2; split.
- apply fx_abs with U; trivial.
- apply typ_abs; trivial.
-Qed.
-
-
-(*************)
-
-
-Lemma impl_natcase : forall o e O P fZ fS n T,
-       isOrd o ->
-       typ_mono e O (Ord o) ->
-       sub_typ (tenv e) (App P n) T -> 
-       typ_impl e fZ (App P Zero) ->
-       typ_impl (push_var e (NatI O)) fS
-         (App (lift 1 P) (App (SuccI (lift 1 O)) (Ref 0))) ->
-       typ_impl e n (NatI (OSucc O)) ->
-       typ_impl e (Natcase fZ fS n) T.
-intros.
-destruct H0.
-destruct H2.
-destruct H3.
-simpl in H7.
-destruct H4.
-split.
- apply Natcase_fx_eq with o O; trivial.
-
- apply typ_natcase' with o O P; trivial.
-Qed.
-
-
-  Lemma impl_call : forall e n x t u T,
+  Lemma typ_inv_rec_call : forall e n x t u T,
     ords e n = false ->
     fixs e n = Some t ->
     t <> kind ->
     u <> kind ->
     nth_error (tenv e) n = value (Prod t u) ->
     sub_typ (tenv e) (subst x (lift1 (S n) u)) T ->
-    typ_impl e x (lift (S n) t) ->
-    typ_impl e (App (Ref n) x) T.
+    typ_inv e x (lift (S n) t) ->
+    typ_inv e (App (Ref n) x) T.
 intros.
-destruct H5.
-assert (typ (tenv e) (Ref n) (Prod (lift (S n) t) (lift1 (S n) u))).
- apply typ_var0; rewrite H3; split;[discriminate|].
- apply sub_refl.
- unfold lift; rewrite eq_lift_prod.
- reflexivity.
-split.
- apply fx_eq_rec_call with t (lift1 (S n) u); trivial.
+apply typ_inv_subsumption with (2:=H4).
+ eapply typ_ext_app with (3:=H5).
+  destruct t as [(t,tm)|]; simpl; trivial; discriminate.
 
- apply typ_subsumption with (subst x (lift1 (S n) u)); auto.
- 2:destruct u as [(u,um)|]; trivial.
- 2:discriminate.
- apply typ_app with (lift (S n) t); trivial.
- destruct t as [(t,tm)|]; trivial.
- discriminate.
-Qed.
+  eapply typ_ext_ref with (4:=H3); trivial.
 
-
-Lemma typ_nat_fix'' : forall infty e O U M T,
-       isOrd infty ->
-       sub_typ (tenv e) (Prod (NatI O) (subst_rec O 1 U)) T ->
-       typ (tenv e) O (Ord infty) ->
-       typ_mono (push_var (push_ord e (OSucc O)) (NatI (OSucc (Ref 0)))) U kind ->
-       typ_ext (push_fun (push_ord e (OSucc O)) (NatI (Ref 0)) U)
-         M (NatI (OSucc (Ref 1)))
-           (lift1 1 (subst_rec (OSucc (Ref 0)) 1 (lift_rec 1 2 U))) ->
-       typ (tenv e) (NatFix O M) T.
-intros.
-destruct H2; destruct H3.
-apply typ_subsumption with (2:=H0).
-2:discriminate.
-apply typ_nat_fix with infty; trivial.
-Qed.
-
-  Lemma typ_ext_fix : forall eps e O U M,
-    isOrd eps ->
-    typ_mono e O (Ord eps) ->
-    typ_ext (push_fun (push_ord e (OSucc O)) (NatI (Ref 0)) U) M
-      (NatI (OSucc (Ref 1))) (lift1 1 (subst_rec (OSucc (Ref 0)) 1 (lift_rec 1 2 U))) ->
-    fx_sub (push_var (push_ord e (OSucc O)) (NatI (OSucc (Ref 0)))) U ->
-    typ_ext e (NatFix O M) (NatI O) (subst_rec O 1 U).
-intros eps e O U M eps_ord tyO tyM tyU.
-destruct tyO as (inclO,tyO).
-destruct tyM as (extM,tyM).
-assert (tyF: typ (tenv e) (NatFix O M) (Prod (NatI O) (subst_rec O 1 U))).
- apply typ_nat_fix with eps; trivial.
-split; trivial.
-apply nat_fix_extend with eps U; trivial.
-Qed.
-
-  Lemma typ_impl_fix : forall eps e O U M,
-    isOrd eps ->
-    typ_impl e O (Ord eps) ->
-    typ_ext (push_fun (push_ord e (OSucc O)) (NatI (Ref 0)) U) M
-      (NatI (OSucc (Ref 1))) (lift1 1 (subst_rec (OSucc (Ref 0)) 1 (lift_rec 1 2 U))) ->
-    fx_sub (push_var (push_ord e (OSucc O)) (NatI (OSucc (Ref 0)))) U ->
-    typ_impl e (NatFix O M) (Prod (NatI O) (subst_rec O 1 U)).
-intros eps e O U M eps_ord tyO tyM tyU.
-destruct tyO as (inclO,tyO).
-destruct tyM as (extM,tyM).
-assert (tyF: typ (tenv e) (NatFix O M) (Prod (NatI O) (subst_rec O 1 U))).
- apply typ_nat_fix with eps; trivial.
-split; trivial.
-apply nat_fix_equals with eps U; trivial.
+ destruct u as [(u,um)|]; simpl; trivial; discriminate.
 Qed.
 
 
@@ -1326,19 +1504,19 @@ Qed.
 
 Section Example.
 
-Definition nat_ind_typ :=
-   Prod (Prod (NatI (Ord omega)) prop) (* P : nat -> Prop *)
+Definition nat_ind_typ K :=
+   Prod (Prod (NatI Infty) K) (* P : nat -> Prop *)
   (Prod (App (Ref 0) Zero)
-  (Prod (Prod (NatI (Ord omega)) (Prod (App (Ref 2) (Ref 0))
-                        (App (Ref 3) (App (SuccI (Ord omega)) (Ref 1)))))
-  (Prod (NatI (Ord omega)) (App (Ref 3) (Ref 0))))).
+  (Prod (Prod (NatI Infty) (Prod (App (Ref 2) (Ref 0))
+                        (App (Ref 3) (App (SuccI Infty) (Ref 1)))))
+  (Prod (NatI Infty) (App (Ref 3) (Ref 0))))).
 
-Definition nat_ind :=
-   Abs (*P*)(Prod (NatI (Ord omega)) prop) (* P : nat -> Prop *)
+Definition nat_ind K :=
+   Abs (*P*)(Prod (NatI Infty) K) (* P : nat -> Prop *)
   (Abs (*fZ*) (App (Ref 0) Zero)
-  (Abs (*fS*) (Prod (*n*)(NatI (Ord omega)) (Prod (App (Ref 2) (Ref 0))
-                                   (App (Ref 3) (App (SuccI (Ord omega)) (Ref 1)))))
-  (NatFix (Ord omega)
+  (Abs (*fS*) (Prod (*n*)(NatI Infty) (Prod (App (Ref 2) (Ref 0))
+                                   (App (Ref 3) (App (SuccI Infty) (Ref 1)))))
+  (NatFix Infty
     (*o,Hrec*)
     (Abs (*n*)(NatI (OSucc (Ref 1)))
       (Natcase
@@ -1347,197 +1525,216 @@ Definition nat_ind :=
                   (App (Ref 2) (Ref 0)))
         (Ref 0)))))).
 
-
-
-Lemma nat_ind_def :
-  forall e, typ e nat_ind nat_ind_typ.
-assert (eq_term Nat (NatI (Ord omega))).
+Lemma nat_ind_def e K (cK:forall f, noccur(B.cons false f)K) :
+  typ_inv e (nat_ind K) (nat_ind_typ K).
+assert (eq_term Nat (NatI Infty)).
  red; simpl.
  red; unfold NAT; reflexivity.
-unfold nat_ind, nat_ind_typ; intros.
-apply typ_abs; try discriminate.
-apply typ_abs; try discriminate.
-apply typ_abs; try discriminate.
-
-set (E0 := Prod (NatI (Ord omega))
-                 (Prod (App (Ref 2) (Ref 0))
-                    (App (Ref 3) (App (SuccI (Ord omega)) (Ref 1))))
-               :: App (Ref 0) Zero :: Prod (NatI (Ord omega)) prop :: e) in |-*.
-change E0 with (tenv (tinj E0)).
-apply typ_nat_fix'' with (osucc omega) (App (Ref 4) (Ref 0)); auto.
- (* sub *)
- apply sub_refl.
- apply eq_typ_prod.
-  reflexivity.
-
-  eapply eq_typ_morph;[reflexivity| |reflexivity].
-  simpl; do 2 red; simpl; intros.
-  unfold V.lams, V.shift; simpl.
-  apply cc_app_morph; apply H0.
-
- (* ord *)
- red; simpl; intros.
- apply lt_osucc; trivial.
+unfold nat_ind, nat_ind_typ.
+apply typ_inv_abs; try discriminate.
+ apply var_eq_noc; noc_tac.
+ trivial.
+(* *)
+apply typ_inv_abs; try discriminate.
+ apply var_eq_noc; noc_tac.
+(* *)
+apply typ_inv_abs; try discriminate.
+ apply var_eq_noc; noc_tac.
+(* *)
+assert (e1 : eq_term (App (Ref 3) (Ref 0)) (subst_rec Infty 1 (App (Ref 4) (Ref 0)))).
+ simpl.
+ red; intros.
+ unfold V.lams, V.shift; simpl.
+ apply cc_app_morph; apply H0.
+rewrite e1.
+apply typ_inv_fix; auto.
+ (* infty : infty *)
+ apply typ_Infty.
+ red; reflexivity.
 
  (* codom mono *)
- split.
-  apply fx_equals_sub.
-  apply fx_eq_noc.
-  apply noc_app.
-   apply noc_var; reflexivity.
-   apply noc_var; reflexivity.
-
-  red; intros; simpl; exact I.
+ Focus 2.
+ apply var_eq_sub.
+ apply var_eq_noc.
+ noc_tac.
 
  (* fix body *)
- apply ext_abs; try discriminate.
-  apply NATi_fx_sub with (o:=osucc (osucc omega)); auto.
-  apply OSucc_fx_sub; auto.
-  apply typ_var_mono with (OSucc (Ord omega)); auto; try discriminate.
-  red; simpl; intros; trivial.
+ apply typ_ext_abs; try discriminate.
+  apply var_mono_NATi.
+   apply typ_OSucc.
+   apply typ_ord_ref with (OSucc Infty); auto.
+    discriminate.
+    red; simpl; auto.
 
-  apply impl_natcase with (osucc omega) (Ref 2) (Ref 5); auto.
-   eapply typ_var_mono.
+   apply var_mono_OSucc.
+   apply var_mono_ref; reflexivity.
+
+  apply typ_inv_natcase with (Ref 2) (Ref 5); auto.
+   eapply typ_ord_ref.
+    simpl; reflexivity.
+    discriminate.
+    red; simpl; auto.
+
+   apply var_mono_ref; simpl; reflexivity.
+
+   (* eqtrm *)
+   simpl tenv; apply sub_refl.
+   red; simpl; intros; reflexivity.
+
+   (* branch 0 *)
+   eapply typ_inv_ref'.
     compute; reflexivity.
     simpl; reflexivity.
     discriminate.
 
-    simpl tenv; apply sub_refl.
-    red; simpl; intros; reflexivity.
-
-   simpl tenv.
-   apply sub_refl.
-   red; simpl; intros.
-   unfold V.lams, V.shift; simpl.
-   reflexivity.
-
-   (* branch 0 *)
-   eapply typ_var_impl.
-    compute; reflexivity.
-    simpl nth_error.
-    reflexivity.
-    discriminate.
-
+    (* eqtrm *)
     apply sub_refl; red; simpl; intros.
-    unfold V.lams, V.shift; simpl.
-    reflexivity.
+    unfold V.lams, V.shift; simpl; reflexivity.
 
    (* branch S *)
-   apply impl_app with (App (Ref 6) (Ref 0))
-     (App (Ref 7) (App (SuccI (Ref 4)) (Ref 1))); try discriminate.
+   apply typ_inv_app with (App (Ref 6) (Ref 0))
+     (App (Ref 7) (App (SuccI Infty) (Ref 1))); try discriminate.
     simpl tenv.
     apply sub_refl; red; intros; simpl.
+    (* conversion (succ domain) *)
     unfold V.lams, V.shift; simpl.
-    reflexivity.
-
-    apply impl_app with (NatI (Ord omega))
-      (Prod (App (Ref 7) (Ref 0)) (App (Ref 8) (App (SuccI (Ord omega)) (Ref 1))));
-      try discriminate.
-     simpl tenv.
-     unfold subst; rewrite eq_subst_prod.
-     apply sub_typ_covariant.
-      red; simpl; intros; reflexivity.
-
-     apply sub_refl.
-     red; intros; simpl.
-     apply cc_app_morph; [reflexivity|].
-     assert (i 1 ∈ NATi (i 4)).
-      generalize (H0 1 _ (eq_refl _)); simpl.
-      unfold V.lams, V.shift; simpl.
-      trivial.
-     rewrite beta_eq.
-      rewrite beta_eq; auto with *.
-       reflexivity.
-       red; intros; apply inr_morph; trivial.
+    assert (i 0 ∈ NATi (i 3)).
+     generalize (H0 0 _ (eq_refl _)); simpl.
+     unfold V.lams, V.shift; simpl; trivial.
+    rewrite beta_eq.
+     rewrite beta_eq; auto with *.
+     red; intros; apply inr_morph; trivial.
 
       red; intros; apply inr_morph; trivial.
 
-      apply NATi_NAT in H1; trivial.
-      generalize (H0 4 _ (eq_refl _)); simpl; intro.
-      apply isOrd_inv with (osucc omega); auto.
+     apply NATi_NAT in H1; trivial.
+     generalize (H0 3 _ (eq_refl _)); simpl; intro.
+     apply isOrd_inv with (osucc omega); auto.
 
-     eapply typ_var_impl.
+    (**)
+    apply typ_inv_app with (NatI Infty)
+      (Prod (App (Ref 7) (Ref 0)) (App (Ref 8) (App (SuccI Infty) (Ref 1))));
+      try discriminate.
+     (* eqtrm *)
+     apply sub_refl; red; intros; simpl.
+     unfold V.lams, V.shift; simpl.
+     reflexivity.
+
+     eapply typ_inv_ref'.
       compute; reflexivity.
       simpl; reflexivity.
       discriminate.
 
-      apply sub_refl.
-      red; intros; simpl.
-      unfold V.lams, V.shift; simpl.
+      (* eqtrm *)
+      apply sub_refl; red; intros; simpl.
+      unfold V.shift, V.lams, V.shift; simpl.
       reflexivity.
 
-     eapply typ_var_impl.
+     eapply typ_inv_ref'.
       compute; reflexivity.
       simpl; reflexivity.
       discriminate.
 
-      red; intros; simpl.
-      simpl in H1.
+      (* subtyping: nat -> infty *)
+      red; simpl; intros.
       unfold V.lams, V.shift in H1; simpl in H1.
       apply NATi_NAT in H1; trivial.
       generalize (H0 3 _ (eq_refl _)); simpl; intro.
       apply isOrd_inv with (osucc omega); auto.
 
-    eapply impl_call.
+    (**)
+    eapply typ_inv_rec_call.
      compute; trivial.
      simpl; reflexivity.
      discriminate.
      2:simpl; reflexivity.
      discriminate.
 
+     (* eqtrm *)
      apply sub_refl; red; intros; simpl.
      unfold V.lams, V.shift; simpl.
      reflexivity.
 
-     eapply typ_var_impl.
+     eapply typ_inv_ref'.
       compute; reflexivity.
       simpl; reflexivity.
       discriminate.
 
+      (* eqtrm *)
       apply sub_refl; red; intros; simpl.
       reflexivity.
 
    (* Scrutinee *)
-   eapply typ_var_impl.
+   eapply typ_inv_ref'.
     compute; reflexivity.
     simpl; reflexivity.
     discriminate.
 
+    (* eqtrm *)
     apply sub_refl; red; intros; simpl.
     reflexivity.
 Qed.
 
+(*
+Lemma int_abs_eq : forall T M i i',
+  int T i == int T i' ->
+  (forall x, x ∈ int T i -> int M (V.cons x i) == int M (V.cons x i')) ->
+  int (Abs T M) i == int (Abs T M) i'.
+intros.
+simpl.
+apply cc_lam_ext.
+ trivial.
+red; intros.
+transitivity (int M (V.cons x' i)).
+ apply int_morph; auto with *.
+ apply V.cons_morph; trivial.
+ reflexivity.
 
-(* Subtraction *)
+ apply H0.
+ rewrite <- H2; trivial.
+Qed.
+*)
+
+(** Subtraction *)
 
 Definition minus O :=
   NatFix O
     (*o,Hrec*)
-    (Abs (*n*) (NatI (OSucc (Ref 1)))
-    (Abs (*m*) (NatI (Ord omega))
+    (Abs (*n*) (NatI (OSucc (Ref(*o*)1)))
+    (Abs (*m*) (NatI Infty)
     (Natcase
        Zero
        (*n'*)
        (Natcase
          (Ref 2)
          (*m'*)
-         (App (App (Ref 4) (Ref 1)) (Ref 0))
-         (Ref 1))
-       (Ref 1)))).
+         (App (App (Ref(*minus*)4) (Ref(*n'*)1)) (Ref(*m'*)0))
+         (Ref(*m*)1))
+       (Ref(*n*)1)))).
 
-Definition minus_typ O := Prod (NatI O) (Prod (NatI (Ord omega)) (NatI (lift 2 O))).
+Definition minus_typ O := Prod (NatI O) (Prod (NatI Infty) (NatI (lift 2 O))).
 
-
-
-Lemma minus_def :
-  forall e infty O,
-  isOrd infty ->
-  typ e O (Ord infty) ->
-  typ e (minus O) (minus_typ O).
+Lemma typ_inv_fix' : forall e O U M T,
+  sub_typ (tenv e) (Prod (NatI O) (subst_rec O 1 U)) T ->
+  typ_ord (tenv e) O ->
+  var_equals e O ->
+  var_mono (push_var (push_ord e (OSucc O)) (NatI (OSucc (Ref 0)))) U ->
+  typ_ext (push_fun (push_ord e (OSucc O)) (NatI (Ref 0)) U) M
+    (NatI (OSucc (Ref 1))) (lift1 1 (subst_rec (OSucc (Ref 0)) 1 (lift_rec 1 2 U))) ->
+  typ_inv e (NatFix O M) T.
 intros.
+apply typ_inv_subsumption with (2:=H).
+2:discriminate.
+apply typ_inv_fix; trivial.
+Qed.
+
+Lemma minus_def e O :
+  typ_ord (tenv e) O ->
+  var_equals e O ->
+  typ_inv e (minus O) (minus_typ O).
+intros tyO eqO.
 unfold minus, minus_typ.
-change e with (tenv (tinj e)).
-apply typ_nat_fix'' with infty (Prod (NatI (Ord omega)) (NatI (Ref 2))); auto.
+apply typ_inv_fix' with (Prod (NatI Infty) (NatI (Ref 2))); auto.
  (* sub *)
  apply sub_refl.
  apply eq_typ_prod.
@@ -1553,65 +1750,67 @@ apply typ_nat_fix'' with infty (Prod (NatI (Ord omega)) (NatI (Ref 2))); auto.
    unfold V.lams, V.shift; simpl; reflexivity.
 
  (* codom mono *)
- split;[|red; intros; simpl; exact I].
- apply fx_sub_prod.
-  apply fx_eq_noc.
-  red; simpl; reflexivity.
+ apply var_mono_prod.
+  apply var_eq_noc; noc_tac.
 
-  apply NATi_sub with infty; trivial.
-  simpl.
-  apply typ_var0; split; [discriminate|].
-  red; intros; simpl.
-  unfold lift in H2; rewrite int_lift_rec_eq in H2.
-  rewrite V.lams0 in H2.
-  simpl in H2.
-  apply le_lt_trans with (2:=H2); trivial.
-  apply H0.
-  red; intros.
-  generalize (H1 (3+n) _ H3).
-  destruct T as [(T,Tm)|]; simpl; trivial.
+  apply var_mono_NATi; trivial.
+   eapply typ_ord_ref.
+    simpl; reflexivity.
+    discriminate.
 
-  apply var_sub.
-  compute; reflexivity.
+    apply typ_ord_lift; simpl.
+    apply typ_OSucc; trivial.
+
+   apply var_mono_ref.
+   compute; reflexivity.
 
  (* fix body *)
- apply ext_abs; try discriminate.
-  apply NATi_fx_sub with (o:=osucc infty); auto.
-  apply OSucc_fx_sub; auto.
-  eapply typ_var_mono.
-   compute; reflexivity.
-   simpl; reflexivity.
-   discriminate.
-  red; simpl; intros; trivial.
-  apply weakening0 in H0; apply weakeningS with (A:=OSucc O) in H0.
-  apply weakeningS with (A:=Prod(NatI(Ref 0))(Prod(NatI(Ord omega))(NatI(Ref 2)))) in H0.
-  apply H0 in H1.
-  simpl in H1.
-  unfold lift in H1; rewrite int_lift_rec_eq in H1.
-  apply le_lt_trans with (3:=H1); trivial.
+ apply typ_ext_abs; try discriminate.
+  apply var_mono_NATi.
+   apply typ_OSucc.
+   eapply typ_ord_ref.
+    simpl; reflexivity.
+    discriminate.
 
+    apply typ_ord_lift; simpl.
+    apply typ_OSucc; trivial.
+
+   apply var_mono_OSucc; auto.
+   apply var_mono_ref.
+   compute; reflexivity.
+
+ (* 2nd abs *)
  rewrite eq_lift_prod.
  rewrite eq_subst_prod.
  unfold lift1; rewrite eq_lift_prod.
- apply impl_abs.
+ eapply typ_inv_subsumption.
+ apply typ_inv_abs.
+ 5:discriminate.
+  Focus 4.
+  apply sub_refl.
+  apply eq_typ_prod.
+   red; intros; simpl; reflexivity.
+
+   reflexivity.
+
   discriminate.
 
-  red; intros; simpl.
-  reflexivity.
+  apply var_eq_noc; noc_tac.
 
-  red; intros; simpl; auto with *.
-
- match goal with |- typ_impl ?e _ _ => set (E:=e) end.
- assert (typ_impl E (Ref 1) (NatI (OSucc (Ref 3)))).
-  eapply typ_var_impl.
-   compute; reflexivity.
+ (**)
+ apply typ_inv_natcase with (Ref 3)
+    (Abs (NatI (OSucc (Ref 3))) (NatI (OSucc (Ref 4)))); auto.
+  eapply typ_ord_ref.
    simpl; reflexivity.
    discriminate.
-  apply sub_refl.
-  red; intros; simpl; reflexivity.
- apply impl_natcase with infty (Ref 3)
-    (Abs (NatI (OSucc (Ref 3))) (NatI (OSucc (Ref 4)))); auto.
-  Focus 2.
+
+   apply typ_ord_lift; simpl.
+   apply typ_OSucc; trivial.
+
+  apply var_mono_ref.
+  compute; reflexivity.
+
+  (* conversion *)
   apply sub_refl.
   rewrite eq_typ_betar.
   3:discriminate.
@@ -1619,58 +1818,39 @@ apply typ_nat_fix'' with infty (Prod (NatI (Ord omega)) (NatI (Ref 2))); auto.
    unfold V.lams, V.shift; simpl.
    reflexivity.
 
-   apply H1.
-
-  (* ord *)
-  eapply typ_var_mono.
-   compute;reflexivity.
-   simpl; reflexivity.
-   discriminate.
-  red; intros; simpl.
-  unfold lift in H3; rewrite int_lift_rec_eq in H3.
-  rewrite V.lams0 in H3.
-  simpl in H3.
-  apply le_lt_trans with (2:=H3); trivial.
-  apply H0.
-  red; intros.
-  generalize (H2 (4+n) _ H4).
-  destruct T as [(T,Tm)|]; simpl; auto.
+   apply typ_var0; split; [discriminate|].
+   apply sub_refl.
+   red; simpl; reflexivity.
 
   (* branch 0 *)
-  split.
-   red; intros; simpl; reflexivity.
-  assert (tyz : typ (tenv E) Zero (NatI (OSucc (Ref 3)))).
-    apply typ_Zero with infty; trivial.
-    apply typ_var0; split; [discriminate|].
-    red; intros; simpl.
-    unfold lift in H3; rewrite int_lift_rec_eq in H3.
-    rewrite V.lams0 in H3.
-    simpl in H3.
-    apply le_lt_trans with (2:=H3); trivial.
-    apply H0.
-    red; intros.
-    generalize (H2 (4+n) _ H4).
-    destruct T as [(T,Tm)|]; simpl; trivial.
-  apply typ_conv with (NatI (OSucc (Ref 3))); trivial.
-  2:discriminate.
-  rewrite eq_typ_betar; trivial.
-  2:discriminate.
-  red; intros; simpl.
-  reflexivity.
-
-  (* branch S *)
-  assert (typ_impl (push_var E (NatI (Ref 3))) (Ref 1) (NatI (Ord (osucc omega)))).
-   eapply typ_var_impl.
-    compute; reflexivity.
+  eapply typ_inv_subsumption.
+   apply typ_inv_Zero.
+   eapply typ_ord_ref with (n:=3).
     simpl; reflexivity.
     discriminate.
+    apply typ_ord_lift; simpl.
+    apply typ_OSucc; trivial.
+
+   2:discriminate.
    apply sub_refl.
-   red; intros; simpl.
-   unfold NATi at 2; rewrite TI_mono_succ; auto.
-   apply NAT_eq.
-  apply impl_natcase with (osucc omega) (Ord omega)
-     (Abs (NatI (OSucc (Ord omega))) (NatI (OSucc (Ref 5)))); auto.
-   Focus 2.
+   rewrite eq_typ_betar.
+   3:discriminate.
+    red; simpl; reflexivity.
+
+    apply typ_Zero.
+    eapply typ_ord_ref.
+     simpl; reflexivity.
+     discriminate.
+     apply typ_ord_lift; simpl.
+     apply typ_OSucc; trivial.
+
+  (* branch S *)
+  apply typ_inv_natcase with Infty
+     (Abs (NatI (OSucc Infty)) (NatI (OSucc (Ref 5)))); auto.
+   apply typ_Infty.
+
+   red; simpl; reflexivity.
+
    apply sub_refl.
    rewrite eq_typ_betar.
    3:discriminate.
@@ -1678,69 +1858,73 @@ apply typ_nat_fix'' with infty (Prod (NatI (Ord omega)) (NatI (Ref 2))); auto.
     rewrite eq_typ_betar.
     3:discriminate.
      red; intros; simpl; reflexivity.
+
      apply typ_conv with (NatI (OSucc (lift_rec 1 0 (Ref 3)))).
      3:discriminate.
-      apply typ_SuccI with (o:=infty); trivial.
-      apply typ_var0; split;[discriminate|].
-      red; intros; simpl.
-      unfold lift in H4; rewrite int_lift_rec_eq in H4.
-      rewrite V.lams0 in H4.
-      simpl in H4.
-      apply le_lt_trans with (2:=H4); trivial.
-      apply H0.
-      red; intros.
-      generalize (H3 (5+n) _ H5).
-      destruct T as [(T,Tm)|]; simpl; trivial.
+      apply typ_app_SuccI; trivial.
+       apply typ_ord_lift; simpl.
+       eapply typ_ord_ref.
+        simpl; reflexivity.
+        discriminate.
+        apply typ_ord_lift; simpl.
+        apply typ_OSucc; trivial.
 
-      apply typ_var0; split;[discriminate|].
-      apply sub_refl; red; intros; simpl.
-      reflexivity.
+       apply typ_var0; split;[discriminate|].
+       apply sub_refl; red; intros; simpl.
+       reflexivity.
 
      red; intros; simpl.
      reflexivity.
 
-     apply H2.
-
-   (* ord *)
-   split.
-    red; intros; simpl; reflexivity.
-
-    red; intros; simpl.
-    apply lt_osucc; trivial.
+    apply typ_var0; split;[discriminate|].
+    (* subtyping infty < infty+ *)
+    red; simpl; intros.
+    revert H0; apply TI_incl; auto with *.
 
   (* branch 0 *)
-  eapply typ_var_impl.
+  eapply typ_inv_ref'.
    compute; reflexivity.
    simpl; reflexivity.
    discriminate.
-  apply sub_refl.
-  rewrite eq_typ_betar.
-  3:discriminate.
-   red; intros; simpl.
-   unfold V.lams, V.shift; simpl; reflexivity.
 
-   eapply typ_Zero with (osucc omega); auto.
-   red; intros; simpl.
-   apply lt_osucc; trivial.
-
-  (* branch S *)    
-  apply impl_app with (NatI (Ord omega)) (NatI (OSucc (Ref 6))).
-   discriminate.
-   discriminate.
-
-   unfold lift; rewrite eq_lift_abs.
    apply sub_refl.
    rewrite eq_typ_betar.
    3:discriminate.
     red; intros; simpl.
-    unfold V.lams, V.shift; simpl.
-    reflexivity.
+    unfold V.lams, V.shift; simpl; reflexivity.
 
-    apply typ_conv with (NatI (OSucc (lift_rec 1 0 (Ord omega)))).
+    eapply typ_Zero; auto.
+    apply typ_Infty.
+
+  (* branch S *)    
+  apply typ_inv_app with (NatI Infty) (NatI (Ref 6)).
+   discriminate.
+   discriminate.
+
+   unfold lift; rewrite eq_lift_abs.
+   apply sub_trans with (NatI (OSucc (Ref 5))).
+    (* sub nat(o) < nat(o+) *)
+    red; simpl; intros.
+    unfold V.lams, V.cons, V.shift in H; simpl in H0.
+    assert (isOrd (i 5)).
+     assert (h := H 5 _ (refl_equal _)); simpl in h.
+     apply isOrd_inv with (2:=h).
+     apply isOrd_succ.
+     rewrite <- int_lift_rec_eq.
+     revert H; apply typ_ord_lift; simpl; trivial.
+    revert H0; apply TI_incl; auto with *.
+
+    apply sub_refl.
+    rewrite eq_typ_betar.
     3:discriminate.
-     apply typ_SuccI with (o:=osucc omega); auto.
-      red; intros; simpl.
-      apply lt_osucc; trivial.
+     red; intros; simpl.
+     unfold V.lams, V.shift; simpl.
+     reflexivity.
+
+     apply typ_conv with (NatI (OSucc (lift_rec 1 0 Infty))).
+     3:discriminate.
+      apply typ_app_SuccI; auto.
+       apply typ_Infty.
 
       apply typ_var0; split;[discriminate|].
       apply sub_refl; red; intros; simpl.
@@ -1749,53 +1933,52 @@ apply typ_nat_fix'' with infty (Prod (NatI (Ord omega)) (NatI (Ref 2))); auto.
      red; intros; simpl.
      reflexivity.
 
-   eapply impl_call.
+   eapply typ_inv_rec_call.
     compute; reflexivity.
     simpl; reflexivity.
     discriminate.
     2:simpl; reflexivity.
     discriminate.
 
+    apply sub_refl.
     unfold subst, lift1; rewrite eq_lift_prod.
     rewrite eq_subst_prod.
-    apply sub_typ_covariant.
-     red; intros; simpl; reflexivity.
+    red; intros; simpl; reflexivity.
 
-     red; intros; simpl.
-     rewrite int_subst_rec_eq in H4.
-     simpl in H4; unfold V.lams, V.shift in H4; simpl in H4.
-     assert (isOrd (i 6)).
-      generalize (H3 6 _ (reflexivity _)).
-      simpl; intro.
-      rewrite V.lams0 in H5.
-      apply isOrd_inv with (2:=H5).      
-      apply isOrd_succ.
-      assert (val_ok e (V.shift 7 i)).
-       red; intros.
-       generalize (H3 (7+n) _ H6).
-       destruct T as [(T,Tm)|]; simpl; auto.
-      apply H0 in H6.
-      simpl in H6.
-      apply isOrd_inv with infty; trivial.
-     revert H4; apply TI_incl; auto.
-
-    eapply typ_var_impl.
+    eapply typ_inv_ref'.
      compute; reflexivity.
      simpl; reflexivity.
      discriminate.
 
      apply sub_refl.
-     red; intros; simpl.
-     reflexivity.
+     red; intros; simpl; reflexivity.
 
-     eapply typ_var_impl.
+     eapply typ_inv_ref'.
       compute; reflexivity.
       simpl; reflexivity.
       discriminate.
 
       apply sub_refl.
-      red; intros; simpl.
-      reflexivity.
+      red; intros; simpl; reflexivity.
+
+   (**)
+   eapply typ_inv_ref'.
+    compute; reflexivity.
+    simpl; reflexivity.
+    discriminate.
+
+    (* infty < infty+ *)
+    red; simpl; intros.
+    revert H0; apply TI_incl; auto with *.
+
+  (**)
+  eapply typ_inv_ref'.
+   compute; reflexivity.
+   simpl; reflexivity.
+   discriminate.
+
+   apply sub_refl.
+   red; intros; simpl; reflexivity.
 Qed.
 
 End Example.
