SN_CIC.v
@@ -1,0 +1,2505 @@
+Require Import List Bool Models.
+Require SN_CC_Real.
+Import ZFgrothendieck.
+Import ZF ZFsum ZFnats ZFrelations ZFord ZFfix.
+Require Import ZFfunext ZFfixrec ZFecc ZFind_nat.
+
+Import SN_CC_Real.
+Import SN_CC_Real.CCSN.
+Import SN_CC_Real.SN.
+Opaque Real.
+Import Sat Sat.SatSet.
+
+Lemma Real_intro x t T :
+  x ∈ El T ->
+  (x ∈ El T -> inSAT t (Real T x)) ->
+  [x,t] \real T.
+split; auto.
+Qed.
+
+Lemma Real_ax x t T R :
+  (forall x x', x ∈ T -> x==x' -> eqSAT (R x) (R x')) ->
+  ([x,t] \real mkTY T R <-> x ∈ T /\ inSAT t (R x)).
+intros.
+unfold inX; rewrite El_def.
+split; destruct 1; split; trivial; rewrite Real_def in *; auto with *.
+Qed.
+
+Lemma Real_intro2 x t T R :
+  (forall x x', x ∈ T -> x==x' -> eqSAT (R x) (R x')) ->
+  x ∈ T ->
+  (x ∈ T -> inSAT t (R x)) ->
+  [x,t] \real mkTY T R.
+split.
+ unfold inX; rewrite El_def; trivial.
+
+ rewrite Real_def; auto.
+Qed.
+
+
+(** Derived rules of the basic judgements *)
+
+Lemma eq_typ_betar : forall e N T M,
+  typ e N T ->
+  T <> kind ->
+  eq_typ e (App (Abs T M) N) (subst N M).
+intros.
+apply eq_typ_beta; trivial.
+ reflexivity.
+ reflexivity.
+Qed.
+
+Lemma typ_var0 : forall e n T,
+  match T, nth_error e n with
+    Some _, value T' => T' <> kind /\ sub_typ e (lift (S n) T') T
+  | _,_ => False end ->
+  typ e (Ref n) T.
+intros.
+case_eq T; intros.
+ rewrite H0 in H.
+case_eq (nth_error e n); intros.
+ rewrite H1 in H.
+ destruct H.
+ apply typ_subsumption with (lift (S n) t); auto.
+  apply typ_var; trivial.
+
+  destruct t as [(t,tm)|]; simpl; try discriminate.
+  elim H; trivial.
+
+  discriminate.
+
+ rewrite H1 in H; contradiction.
+ rewrite H0 in H; contradiction.
+Qed.
+
+
+(** Subtyping *)
+
+Definition sub_typ_covariant : forall e U1 U2 V1 V2,
+  U1 <> kind ->
+  eq_typ e U1 U2 ->
+  sub_typ (U1::e) V1 V2 ->
+  sub_typ e (Prod U1 V1) (Prod U2 V2).
+intros.
+apply sub_typ_covariant; trivial.
+intros.
+unfold eqX, lam, app.
+unfold inX in H2.
+unfold prod in H2; rewrite El_def in H2.
+apply cc_eta_eq in H2; trivial.
+Qed.
+
+(** Universes *)
+(*Module Lc:=Lambda.
+Definition type (n:nat) : trm :=
+  cst (mkTY (ecc n) (fun _ => snSAT)) Lc.K (fun _ _ => eq_refl) (fun _ _ _ => eq_refl).
+
+Lemma typ_Prop : forall e, typ e prop (type 0).
+red; intros; simpl.
+split;[discriminate|split].
+ unfold inX; simpl.
+ rewrite El_def.
+ apply (grot_succ_in gr).
+Qed.
+
+Lemma typ_Type : forall e n, typ e (type n) (type (S n)).
+red; intros; simpl.
+apply (grot_succ_in gr).
+Qed.
+
+Lemma cumul_Type : forall e n, sub_typ e (type n) (type (S n)).
+red; simpl; intros.
+red; intros.
+apply ecc_incl; trivial.
+Qed.
+
+Lemma cumul_Prop : forall e, sub_typ e prop (type 0).
+red; simpl; intros.
+red; intros.
+apply G_trans with props; trivial.
+ apply (grot_succ_typ gr).
+
+ apply (grot_succ_in gr).
+Qed.
+
+Lemma typ_prod2 : forall e n T U,
+  typ e T (type n) ->
+  typ (T :: e) U (type n) ->
+  typ e (Prod T U) (type n).
+Proof.
+unfold typ, Prod; simpl; red; intros e n T U ty_T ty_U i is_val.
+apply G_cc_prod.
+ apply ecc_grot.
+
+ red; red; intros.
+ rewrite H0; auto with *.
+
+ apply ty_T; trivial.
+
+ intros.
+ apply ty_U.
+ apply vcons_add_var; auto.
+Qed.
+*)
+
+
+(** Ordinals *)
+
+Definition Ord (o:set) : trm :=
+  cst o Lc.K (fun _ _ => eq_refl) (fun _ _ _ => eq_refl).
+
+Definition Ordt (o:set) : trm :=
+  cst (mkTY o (fun _ => snSAT)) Lc.K (fun _ _ => eq_refl) (fun _ _ _ => eq_refl).
+
+Definition typ_ord_kind : forall e o, zero ∈ o -> typ e (Ordt o) kind.
+red; simpl; intros.
+split; [|split]; simpl.
+ discriminate.
+
+ exists nil; exists (Ordt o);[reflexivity|].
+ exists zero; intros; simpl.
+ unfold inX; rewrite El_def; trivial.
+
+ apply Lc.sn_K.
+Qed.
+
+
+Definition typ_ord_ord : forall e o o',
+  o < o' -> typ e (Ord o) (Ordt o').
+red; simpl; intros.
+apply in_int_intro; try discriminate.
+simpl.
+rewrite Real_ax;[split|]; auto with *.
+apply Lc.sn_K.
+Qed.
+
+
+Definition OSucc : trm -> trm.
+(*begin show*)
+intros o; left; exists (fun i => osucc (int i o)) (fun j => tm j o).
+(*end show*)
+ do 2 red; intros.
+ rewrite H; reflexivity.
+ (**)
+ do 2 red; intros.
+ rewrite H; reflexivity.
+ (**)
+ red; intros.
+ apply tm_liftable.
+ (**)
+ red; intros.
+ apply tm_substitutive.
+Defined.
+
+Definition OSucct : trm -> trm.
+(*begin show*)
+intros o; left; exists (fun i => mkTY (osucc (int i o)) (fun _ => snSAT)) (fun j => tm j o).
+(*end show*)
+ do 2 red; intros.
+ apply mkTY_ext; auto with *.
+ rewrite H; reflexivity.
+ (**)
+ do 2 red; intros.
+ rewrite H; reflexivity.
+ (**)
+ red; intros.
+ apply tm_liftable.
+ (**)
+ red; intros.
+ apply tm_substitutive.
+Defined.
+
+Lemma tyord_inv : forall e i j o o',
+  isOrd o' ->
+  typ e o (Ordt o') ->
+  val_ok e i j ->
+  isOrd (int i o) /\ int i o < o' /\ Lc.sn (tm j o).
+unfold typ; intros.
+specialize H0 with (1:=H1).
+apply in_int_not_kind in H0.
+2:discriminate.
+simpl in H0.
+rewrite Real_ax in H0; auto with *.
+destruct H0.
+eauto using isOrd_inv.
+Qed.
+
+(** Nat *)
+Require Import SATnat.
+
+Definition Nat : trm.
+(*begin show*)
+left; exists (fun _ => mkTY NAT cNAT) (fun _ => Lc.K).
+(*end show*)
+ do 2 red; reflexivity.
+ do 2 red; reflexivity.
+ red; reflexivity.
+ red; reflexivity.
+Defined.
+
+Definition NatI (O:trm) : trm.
+(*begin show*)
+left; exists (fun i => mkTY (NATi (int i O)) cNAT) (fun j => tm j O).
+(*end show*)
+ do 2 red; intros.
+ unfold eqX.
+ apply mkTY_ext.
+  rewrite H; reflexivity.
+
+  intros.
+  apply fam_mrph; trivial.
+  revert H0; apply NATi_NAT.
+  admit.
+ (**)
+ do 2 red; intros.
+ rewrite H; reflexivity.
+ (**)
+ red; intros.
+ apply tm_liftable.
+ (**)
+ red; intros.
+ apply tm_substitutive.
+Defined.
+
+Lemma typ_natI : forall e eps o,
+  isOrd eps ->
+  typ e o (Ordt eps) ->
+  typ e (NatI o) kind.
+red; intros; simpl.
+red in H0; specialize H0 with (1:=H1).
+apply in_int_not_kind in H0.
+2:discriminate.
+split;[|split].
+ discriminate.
+
+ exists nil; exists (NatI o);[reflexivity|].
+ admit. (* not empty *)
+
+ simpl.
+ apply real_sn in H0; trivial.
+Qed.
+
+Lemma realNati_def x t i O :
+ isOrd (int i O) ->
+ ([x,t] \real int i (NatI O) <->
+  x ∈ NATi (int i O) /\ inSAT t (cNAT x)).
+intros.
+simpl.
+rewrite Real_ax; auto with *.
+intros.
+apply fam_mrph; trivial.
+revert H0; apply NATi_NAT; trivial.
+Qed.
+
+(* Zero *)
+
+
+Definition Zero : trm.
+(* begin show *)
+left; exists (fun _ => ZERO) (fun _ => ZE).
+(* end show *)
+ do 2 red; reflexivity.
+ do 2 red; reflexivity.
+ red; reflexivity.
+ red; reflexivity.
+Defined.
+
+Lemma typ_Zero : forall o e O,
+  isOrd o ->
+  typ e O (Ordt o) ->
+  typ e Zero (NatI (OSucc O)).
+red; simpl; intros.
+destruct tyord_inv with (2:=H0)(3:=H1) as (?,(?,_)); trivial.
+apply in_int_intro; try discriminate.
+rewrite realNati_def.
+2:simpl; auto.
+split.
+ simpl.
+ apply ZEROi_typ; trivial.
+
+ simpl tm.
+ apply cNAT_ZE.
+Qed.
+
+
+(* Successor *)
+
+Definition Succ (o:trm): trm.
+(* begin show *)
+left; exists (fun i => lam (int i (NatI o)) SUCC) (fun _ => SU).
+(*end show *)
+ do 2 red; intros.
+ apply lam_ext.
+  apply mkTY_ext; auto with *.
+   rewrite H; reflexivity.
+
+   intros.
+   apply fam_mrph; trivial.
+   revert H0; apply NATi_NAT.
+   admit. (* ord *)
+
+  red; intros.
+  rewrite H1; reflexivity.
+
+ do 2 red; auto.
+
+ red; reflexivity.
+
+ red; reflexivity.
+Defined.
+
+
+Lemma El_prod A Ar B Br :
+  ext_fun A B ->
+  El (prod(mkTY A Ar) (fun x => mkTY (B x) (Br x))) ==
+  cc_prod A B.
+intros.
+unfold prod; rewrite El_def.
+apply cc_prod_ext.
+ rewrite El_def; reflexivity.
+
+ red; intros.
+ rewrite El_def; apply H; trivial.
+ rewrite El_def in H0; trivial.
+Qed.
+(*
+ Lemma prodReal :
+  [x,t] \real prod (mkTY A Ar) (fun x => mkTY (B x) (Br x)) <->
+  x ∈ cc_prod
+*)
+
+Lemma typ_succi : forall e o i,
+  isOrd o ->
+  typ e i (Ordt o) ->
+  typ e (Succ i) (Prod (NatI i) (NatI (OSucc (lift 1 i)))). 
+red; intros.
+destruct tyord_inv with (2:=H0) (3:=H1) as (?,(?,?)); trivial.
+clear H0.
+apply in_int_intro; try discriminate.
+apply prod_intro_sn.
+ red; intros.
+ rewrite H5; reflexivity.
+
+ red; intros.
+ rewrite H5; reflexivity.
+
+ simpl.
+ unfold SU.
+ constructor; intros.
+ red in H0; apply Lc.nf_norm in H0; [contradiction|].
+ repeat constructor.
+
+ intros.
+ rewrite realNati_def in H0 |- *; auto with *.
+ 2:simpl;rewrite int_lift_eq; simpl; auto.
+ destruct H0.
+ split.
+  simpl; rewrite int_lift_eq; simpl.
+  apply SUCCi_typ; auto.
+
+  apply cNAT_SU; trivial.
+  revert H0; apply NATi_NAT; auto.
+Qed.
+
+(* Case analysis *)
+
+Definition Natcase (fZ fS n : trm) : trm.
+(*begin show*)
+left; exists (fun i => NATCASE (int i fZ) (fun k => int (V.cons k i) fS) (int i n))
+       (fun j => NCASE (tm j fZ) (Lc.Abs (tm (Lc.ilift j) fS)) (tm j n)).
+(*end show*)
+do 2 red; intros.
+red.
+apply NATCASE_morph.
+ rewrite H; reflexivity.
+ red; intros.
+ rewrite H; rewrite H0; reflexivity.
+ rewrite H; reflexivity.
+(**)
+admit.
+admit.
+admit.
+(* red; intros.
+ rewrite H; rewrite H0; reflexivity.
+(**)
+ rewrite H; reflexivity.*)
+Defined.
+
+Instance Natcase_morph :
+  Proper (eq_trm ==> eq_trm ==> eq_trm ==> eq_trm) Natcase.
+do 4 red; intros.
+split; red; simpl; intros.
+ apply NATCASE_morph_gen; intros.
+  rewrite H1; rewrite H2; reflexivity.
+  rewrite H; rewrite H2; reflexivity.
+  rewrite H0; rewrite H4; rewrite H2; reflexivity.
+
+ rewrite H; rewrite H0; rewrite H1; rewrite H2; trivial.
+Qed.
+
+Notation "'int0' x y" := (int y x) (at level 10, x at level 9, y at level 9).
+
+Lemma Natcase_succ : forall o O e n fZ fS,
+  isOrd o ->
+  typ e O (Ordt o) ->
+  typ e n (NatI O) ->
+  eq_typ e (Natcase fZ fS (App (Succ O) n)) (subst n fS).
+red; intros.
+destruct tyord_inv with (2:=H0) (3:=H2) as (?,(?,_)); trivial.
+(*red in H0; specialize H0 with (1:=H2).*)
+red in H1; specialize H1 with (1:=H2).
+(*apply in_int_not_kind in H0.
+2:discriminate.
+destruct H0 as (H0,_).*)
+apply in_int_not_kind in H1.
+2:discriminate.
+rewrite realNati_def in H1; trivial.
+destruct H1 as (H1,_).
+red; simpl.
+rewrite <- (fun e1 e2 => NATCASE_morph (int0 fZ i) (int0 fZ i) e1
+  (fun k => int0 fS (V.cons k i)) (fun k => int0 fS (V.cons k i)) e2
+  (SUCC (int0 n i))); auto with *.
+ rewrite NATCASE_SUCC; auto.
+  rewrite int_subst_eq; reflexivity.
+
+  intros.
+  rewrite H5; reflexivity.
+
+ red; intros.
+ rewrite H5; reflexivity.
+
+ rewrite beta_eq; auto with *.
+  red; intros.
+  unfold SUCC; apply inr_morph; trivial.
+
+  rewrite El_def; trivial.
+Qed.
+Existing Instance NATi_morph.
+
+Lemma typ_natcase : forall o e O P fZ fS n,
+  isOrd o ->
+  typ e O (Ordt o) ->
+  typ e fZ (App P Zero) ->
+  typ (NatI O :: e) fS (App (lift 1 P) (App (Succ (lift 1 O)) (Ref 0))) ->
+  typ e n (NatI (OSucc O)) ->
+  typ e (Natcase fZ fS n) (App P n).
+red; intros.
+destruct tyord_inv with (2:=H0)(3:=H4) as (?,(?,_ )); trivial.
+red in H1; specialize H1 with (1:=H4).
+apply in_int_not_kind in H1;[|discriminate].
+red in H3; specialize H3 with (1:=H4).
+apply in_int_not_kind in H3;[|discriminate].
+apply in_int_intro; try discriminate.
+destruct H1.
+rewrite realNati_def in H3; simpl in H3|-*; auto.
+destruct H3.
+apply Real_intro; intros.
+ apply NATCASE_typ with (o:=int i O) (P:=fun n => El(app (int i P) n)); intros; trivial.
+  do 2 red; intros.
+  rewrite H9; reflexivity.
+
+  do 2 red; intros.
+  rewrite H9; reflexivity.
+
+  assert (val_ok (NatI O :: e) (V.cons n0 i) (I.cons daimon j)).
+   apply vcons_add_var; trivial.
+   2:discriminate.
+   rewrite realNati_def; auto with *.
+   split; trivial.
+   apply varSAT.
+  apply H2 in H10; clear H1; simpl in H10.
+  apply in_int_not_kind in H10;[|discriminate].
+  destruct H10 as(H10,_ ).
+  revert H10; apply eq_elim; simpl.
+  rewrite int_cons_lift_eq.
+  rewrite beta_eq; auto with *.
+   red; intros; apply inr_morph; auto.
+
+   rewrite El_def.
+   rewrite int_cons_lift_eq; trivial.
+
+ rewrite cNAT_eq in H8.
+ pose (B:=fun k => Real (app (int0 P i) k)
+         (NATCASE (int0 fZ i) (fun k => int0 fS (V.cons k i)) k)).
+ assert (Bm : forall x y,  x ∈ NAT -> x == y -> eqSAT (B x) (B y)).
+  unfold B; intros.
+  apply Real_morph.
+   rewrite H11; reflexivity.
+
+   apply NATCASE_morph; auto with *.
+   red; intros.
+   rewrite H12; reflexivity.
+
+ unfold NATi in H3; rewrite TI_mono_succ in H3; auto with *.
+ rewrite fNAT_def in H8.
+ unfold NCASE.
+ apply H8 with (P:=mkFam B Bm).
+  simpl; trivial.
+  unfold B; simpl in H1|-*.
+  rewrite NATCASE_ZERO.
+  trivial.
+
+  rewrite piNAT_ax.
+  split; intros.
+   admit.
+
+   apply prodSAT_intro; intros.
+   unfold Lc.subst; simpl Lc.subst_rec.
+   apply prodSAT_intro; intros.
+   unfold Lc.subst; simpl Lc.subst_rec.
+   rewrite Lc.simpl_subst_rec; auto.
+   rewrite Lc.simpl_subst_rec; auto.
+   rewrite Lc.lift_rec0.
+   rewrite Lc.simpl_subst; auto.
+   rewrite Lc.lift0.
+
+simpl.
+
+ apply NCASE_fNAT with (A:=cNAT) (B:=mkFam B Bm) (k:=int0 n i); trivial.
+  revert H3; apply NATi_NAT; auto.
+
+  unfold B; simpl in H1|-*.
+  rewrite NATCASE_ZERO.
+  trivial.
+  rewrite piNAT_ax.
+  split; intros.
+   apply typ_abs in H2.
+    3:discriminate.
+    2:left.
+    2:apply typ_natI with o; trivial.
+   apply H2 in H4.
+   apply in_int_sn in H4.
+   eapply Lc.subterm_sn.
+   eapply Lc.subterm_sn.
+   eexact H4.
+   apply Lc.sbtrm_app_l.
+   apply Lc.sbtrm_app_r.
+
+   apply prodSAT_intro.
+   intros.
+   trivial.
+   apply in_int_not_kind in H4.
+   2:discriminate.
+   apply Lc.sn_abs.
+
+  assert (val_ok (NatI O :: e) (V.cons (int0 n i) i) (I.cons daimon j)).
+   apply vcons_add_var; trivial.
+   2:discriminate.
+   rewrite realNati_def; auto with *.
+   split; trivial.
+   apply varSAT.
+
+
+Lemma NCASE_fNAT f g n k (A B:family) :
+  k ∈ NAT ->
+  inSAT n (fNAT A k) ->
+  inSAT f (B ZERO) ->
+  inSAT g (piNAT(fun m => prodSAT (A m) (B (SUCC m)))) ->
+  inSAT (NCASE f g n) (B k).
+unfold NCASE; intros.
+rewrite fNAT_def in H0.
+apply H0 with (P:=B); intros; trivial.
+rewrite piNAT_ax in H2|-*; intros.
+destruct H2 as (sng,H2).
+split; intros.
+ do 2 apply Lc.sn_abs.
+ apply sn_app_var.
+ apply Lc.sn_lift; trivial.
+apply prodSAT_intro; intros.
+unfold Lc.subst; simpl Lc.subst_rec.
+apply prodSAT_intro; intros.
+unfold Lc.subst; simpl Lc.subst_rec.
+repeat rewrite Lc.simpl_subst; trivial.
+do 2 rewrite Lc.lift0.
+apply prodSAT_elim with (2:=H4); auto.
+Qed.
+
+
+  exact H1.
+  auto.
+
+impl_int_lift1.
+ in H6; trivial.
+
+   red; intros.
+   unfold SUCC; apply inr_morph; trivial.
+
+   rewrite simpl_int_lift1; auto.*)
+Qed.
+
+Lemma typ_natcase' : forall o e O P fZ fS n T,
+  isOrd o ->
+  T <> kind ->
+  typ e O (Ordt o) ->
+  sub_typ e (App P n) T -> 
+  typ e fZ (App P Zero) ->
+  typ (NatI O :: e) fS
+    (App (lift 1 P) (App (Succ (lift 1 O)) (Ref 0))) ->
+  typ e n (NatI (OSucc O)) ->
+  typ e (Natcase fZ fS n) T.
+intros.
+apply typ_subsumption with (App P n); auto.
+2:discriminate.
+apply typ_natcase with o O; trivial.
+Qed.
+
+(********************************************************************************)
+(** Occurrences *)
+
+
+  (* Non-occurrence : interp do not depend on variables in set [f] *)
+  Definition noccur (f:nat->bool) (T:trm) : Prop :=
+    forall i i',
+    (forall n, if f n then True else i n == i' n) ->
+    int i T == int i' T.
+
+  Lemma noc_var : forall f n, f n = false -> noccur f (Ref n).
+red; simpl; intros.
+specialize (H0 n).
+rewrite H in H0; trivial.
+Qed.
+
+  Lemma noc_kind : forall f, noccur f kind.
+red; simpl; reflexivity.
+Qed.
+
+  Lemma noc_prop : forall f, noccur f prop.
+red; simpl; reflexivity.
+Qed.
+
+  Lemma noc_app : forall f a b,
+    noccur f a -> noccur f b -> noccur f (App a b).
+unfold noccur; simpl; intros.
+rewrite (H _ _ H1).
+rewrite (H0 _ _ H1).
+reflexivity.
+Qed.
+
+
+(********************************************************************************)
+(** Judgements with variance *)
+
+Module Beq.
+Definition t := bool.
+Definition eq := @eq bool.
+Definition eq_equiv : Equivalence eq := eq_equivalence.
+Existing Instance eq_equiv.
+End Beq.
+Module B := VarMap.Make(Beq).
+
+Module OTeq.
+Definition t := option trm.
+Definition eq := @eq (option trm).
+Definition eq_equiv : Equivalence eq := eq_equivalence.
+Existing Instance eq_equiv.
+End OTeq.
+Module OT := VarMap.Make(OTeq).
+
+(* Environments with tags on ordinal and recursive function variables *)
+Record fenv := {
+  tenv : env;
+  ords : B.map; (* variables denoting ordinals *)
+  fixs : OT.map (* variables denoting recursive functions with their domain *)
+}.
+
+Definition tinj e :=
+  Build_fenv e (B.nil false) (OT.nil None).
+
+Definition push_var e T :=
+  Build_fenv (T::tenv e) (B.cons false (ords e)) (OT.cons None (fixs e)).
+
+Definition push_fun e dom rng :=
+  Build_fenv (Prod dom rng::tenv e)
+    (B.cons false (ords e)) (OT.cons (Some dom) (fixs e)).
+
+Definition push_ord e T :=
+  Build_fenv (T::tenv e) (B.cons true (ords e)) (OT.cons None (fixs e)).
+
+
+(* Additional judgments for fix body *)
+Definition val_mono (e:fenv) i j i' j' :=
+    val_ok (tenv e) i j /\
+    val_ok (tenv e) i' j' /\
+    forall n,
+    if ords e n then i n ⊆ i' n
+    else match fixs e n with
+      Some T => forall x, x ∈ El(int (V.shift (S n) i) T) -> app (i n) x == app (i' n) x
+    | _ => i n == i' n
+    end.
+
+Lemma val_mono_refl : forall e i j,
+  val_ok (tenv e) i j -> val_mono e i j i j.
+split;[idtac|split]; simpl; auto with *.
+intro n.
+destruct (ords e n); auto with *.
+destruct (fixs e n); auto with *.
+Qed.
+
+Lemma val_push_var : forall e i j i' j' x t x' t' T,
+  val_mono e i j i' j' ->
+  x == x' ->
+  [x,t] \real int i T ->
+  [x',t'] \real int i' T ->
+  T <> kind ->
+  val_mono (push_var e T) (V.cons x i) (I.cons t j) (V.cons x' i') (I.cons t' j').
+destruct 1 as (?&?&?); split;[idtac|split]; trivial.
+ unfold push_var; simpl.
+ apply vcons_add_var; trivial.
+
+ unfold push_var; simpl.
+ apply vcons_add_var; trivial.
+
+ destruct n as [|n]; simpl; auto.
+ generalize (H1 n).
+ destruct (ords e n); trivial.
+Qed.
+
+Lemma val_push_ord : forall e i j i' j' x t x' t' T,
+  val_mono e i j i' j' ->
+  x ⊆ x' ->
+  [x,t] \real int i T ->
+  [x',t'] \real int i' T ->
+  T <> kind ->
+  val_mono (push_ord e T) (V.cons x i) (I.cons t j) (V.cons x' i') (I.cons t' j').
+destruct 1 as (?&?&?); split;[idtac|split]; trivial.
+ unfold push_ord; simpl.
+ apply vcons_add_var; trivial.
+
+ unfold push_ord; simpl.
+ apply vcons_add_var; trivial.
+
+ destruct n as [|n]; simpl; auto.
+ generalize (H1 n).
+ destruct (ords e n); trivial.
+Qed.
+
+Lemma val_push_fun : forall e i j i' j' f tf g tg T U,
+  val_mono e i j i' j' ->
+  [f,tf] \real prod (int i T) (fun x => int (V.cons x i) U) ->
+  [g,tg] \real prod (int i' T) (fun x => int (V.cons x i') U) ->
+  fcompat (El(int i T)) f g ->
+  val_mono (push_fun e T U) (V.cons f i) (I.cons tf j) (V.cons g i') (I.cons tg j').
+destruct 1 as (?&?&?); split;[idtac|split]; trivial.
+ unfold push_fun; simpl.
+ apply vcons_add_var; trivial.
+ discriminate.
+
+ unfold push_fun; simpl.
+ apply vcons_add_var; trivial.
+ discriminate.
+
+ destruct n as [|n]; simpl; auto.
+ generalize (H1 n).
+ destruct (ords e n); trivial.
+Qed.
+
+(** Function Extension judgment *)
+Definition fx_extends e dom M :=
+  forall i i' j j', val_mono e i j i' j' ->
+  fcompat (El(int i dom)) (int i M) (int i' M).
+
+(** Covariance judgment *)
+Definition fx_sub e M :=
+  forall i i' j j', val_mono e i j i' j' ->
+  forall x t, [x,t] \real int i M -> [x,t] \real int i' M.
+
+Definition fx_subval e M :=
+  forall i i' j j', val_mono e i j i' j' -> int i M ⊆ int i' M.
+
+(** Invariance *)
+Definition fx_equals e M :=
+  forall i i' j j', val_mono e i j i' j' -> int i M == int i' M.
+
+Definition spec_var e n :=
+  ords e n || match fixs e n with Some _ => true | _ => false end.
+
+  Lemma fx_eq_noc : forall e t,
+    noccur (spec_var e) t ->
+    fx_equals e t.
+unfold noccur, fx_equals, spec_var; intros.
+apply H; intros.
+destruct H0 as (_,(_,H0)).
+generalize (H0 n).
+destruct (ords e n); simpl; trivial.
+destruct (fixs e n); simpl; trivial.
+Qed.
+
+  Lemma fx_eq_app : forall e u v,
+    fx_equals e u ->
+    fx_equals e v ->
+    fx_equals e (App u v).
+unfold fx_equals; intros.
+specialize H with (1:=H1).
+specialize H0 with (1:=H1).
+simpl.
+rewrite H; rewrite H0; reflexivity.
+Qed.
+
+  Lemma fx_eq_abs : forall e T M,
+    T <> kind ->
+    fx_equals e T ->
+    fx_equals (push_var e T) M ->
+    fx_equals e (Abs T M).
+unfold fx_equals; intros.
+simpl.
+apply lam_ext; eauto.
+red; intros.
+apply H1 with (I.cons daimon j) (I.cons daimon j').
+specialize H0 with (1:=H2).
+apply val_push_var; auto.
+ split; trivial.
+ apply varSAT.
+
+ split.
+ 2:apply varSAT.
+ unfold inX; rewrite <- H4; rewrite <- H0; trivial.
+Qed.
+
+  Lemma fx_eq_rec_call : forall e n x T U,
+    ords e n = false ->
+    fixs e n = Some T ->
+    T <> kind ->
+    typ (tenv e) (Ref n) (Prod (lift (S n) T) U) ->
+    fx_equals e x ->
+    typ (tenv e) x (lift (S n) T) ->
+    fx_equals e (App (Ref n) x).
+unfold fx_equals; intros.
+simpl.
+specialize H3 with (1:=H5).
+rewrite <- H3.
+destruct H5 as (Hty,(Hty',Hrec)).
+specialize Hrec with n.
+rewrite H in Hrec; rewrite H0 in Hrec.
+apply Hrec.
+red in H4; specialize H4 with (1:=Hty); trivial.
+apply in_int_not_kind in H4; trivial.
+2:destruct T;[discriminate|elim H1;reflexivity].
+destruct H4 as (?,_ ).
+unfold inX in H4.
+unfold lift in H4; rewrite int_lift_rec_eq in H4.
+rewrite V.lams0 in H4; trivial.
+Qed.
+
+  (* Covariance *)
+
+  Lemma fx_equals_subval : forall e M, fx_equals e M -> fx_subval e M.
+unfold fx_subval, fx_equals; intros.
+apply H in H0.
+rewrite <- H0; reflexivity.
+Qed.
+
+  Lemma fx_equals_sub : forall e M, fx_equals e M -> fx_sub e M.
+unfold fx_sub, fx_equals; intros.
+apply H in H0.
+rewrite <- H0; trivial.
+Qed.
+
+  Lemma var_sub : forall e n,
+    ords e n = true ->
+    fx_subval e (Ref n).
+unfold fx_subval; intros.
+destruct H0 as (_,(_,H0)).
+generalize (H0 n); rewrite H.
+simpl; trivial.
+Qed.
+
+Lemma fx_sub_prod : forall e T U,
+  T <> kind ->
+  fx_equals e T ->
+  fx_sub (push_var e T) U ->
+  fx_sub e (Prod T U).
+red; intros.
+rewrite intProd_eq in H3|-*.
+specialize (H0 _ _ _ _ H2).
+destruct H3.
+unfold inX in H3.
+rewrite Real_prod in H4; trivial.
+ unfold prod in H3; rewrite El_def in H3.
+ assert (x ∈ El(prod (int i' T) (fun x0 : X => int (V.cons x0 i') U))).
+  unfold prod, inX; rewrite El_def.
+  revert H3; apply cc_prod_covariant.
+   do 2 red; intros.
+   rewrite H5; reflexivity.
+
+   rewrite H0; reflexivity.
+
+   intros.
+   red in H1.
+   assert (val_mono (push_var e T) (V.cons x0 i) (I.cons daimon j) (V.cons x0 i') (I.cons daimon j')).
+    apply val_push_var; auto with *.
+    split; trivial; apply varSAT.
+    split.
+     rewrite <- H0; trivial.
+     apply varSAT.
+   specialize (H1 _ _ _ _ H5).
+   red; intros.
+   destruct H1 with z daimon; trivial.
+   split; trivial.
+   apply varSAT.
+ split; trivial.
+ rewrite Real_prod; trivial.
+  unfold piSAT.
+  apply interSAT_intro' with
+   (F:=fun v => prodSAT(Real(int i' T) v)(Real(int(V.cons v i') U)(cc_app x v))).
+   apply sat_sn in H4; trivial.
+   intros.
+   rewrite <- H0 in H6.
+   specialize interSAT_elim with (1:=H4) (x:=exist (fun x=>_) x0 H6); simpl proj1_sig; intros.
+   revert H7; apply prodSAT_mono.
+    do 2 red; intros.
+    rewrite <- H0 in H7; trivial.
+
+    red; intros.
+    apply H1 with (i:=V.cons x0 i) (j:=I.cons daimon j) (j':=I.cons daimon j').
+     apply val_push_var; auto with *.
+     split; trivial; apply varSAT.
+     split.
+      rewrite <- H0; trivial.
+      apply varSAT.
+
+     split; trivial.
+     unfold inX; apply cc_prod_elim with (1:=H3); trivial.
+
+  red; intros.
+  rewrite H7; reflexivity.
+
+ red; intros.
+ rewrite H6; reflexivity.
+Qed.
+
+  Lemma NATi_sub : forall e o O,
+    isOrd o ->
+    typ (tenv e) O (Ordt o) ->
+    fx_subval e O ->
+    fx_sub e (NatI O).
+unfold fx_sub, fx_subval; intros.
+destruct tyord_inv with (2:=H0) (3:=proj1 H2); trivial.
+destruct tyord_inv with (2:=H0) (3:=proj1 (proj2 H2)); trivial.
+specialize H1 with (1:=H2).
+rewrite realNati_def in H3|-*; trivial.
+destruct H3.
+split; trivial.
+revert H3; apply TI_mono; auto.
+Qed.
+
+  Lemma OSucc_sub : forall e O,
+    fx_subval e O ->
+    fx_subval e (OSucc O).
+unfold fx_subval; simpl; intros.
+apply osucc_mono; eauto.
+ admit.
+ admit.
+Qed.
+
+  (* Function subtyping *)
+
+  Lemma fx_abs : forall e U T M,
+    T <> kind ->
+    fx_sub e T ->
+    fx_equals (push_var e T) M ->
+    typ (T::tenv e) M U ->
+    U <> kind ->
+    fx_extends e T (Abs T M).
+unfold fx_sub, fx_equals, fx_extends; intros.
+specialize H0 with (1:=H4).
+simpl.
+red; intros.
+fold app.
+rewrite beta_eq; try assumption.
+ rewrite beta_eq.
+  apply H1 with (I.cons daimon j) (I.cons daimon j').
+  apply val_push_var; auto with *.
+   split; [trivial|apply varSAT].
+
+   split; [trivial|apply varSAT].
+   destruct H0 with x daimon; trivial.
+   split; [trivial|apply varSAT].
+
+  red; red; intros.
+  rewrite H7; reflexivity.
+
+  apply H0 with (x:=x) (t:=daimon); trivial.
+  split; [trivial|apply varSAT].
+
+ red; red; intros.
+ rewrite H7; reflexivity.
+Qed.
+
+(*
+Lemma Natcase_fx_eq : forall o e O f1 f2 c,
+  isOrd o ->
+  typ (tenv e) O (Ord o) ->
+  fx_sub e O ->
+  fx_equals e f1 ->
+  fx_equals (push_var e (NatI O)) f2 ->
+  typ (tenv e) c (NatI (OSucc O)) ->
+  fx_equals e c ->
+  fx_equals e (Natcase f1 f2 c).
+red; intros o e O f1 f2 c H tyO H0 H1 H2 tyc H3 i i' H4.
+simpl.
+assert (ord : isOrd (int O i)).
+ destruct H4 as (H4,_); apply tyO in H4.
+ apply isOrd_inv with o; trivial.
+assert (ord' : isOrd (int O i')).
+ destruct H4 as (_,(H4,_)); apply tyO in H4.
+ apply isOrd_inv with o; trivial.
+assert (int c i ∈ NATi (osucc (int O i))).
+ destruct H4 as (H4,_).
+ apply tyc in H4; trivial.
+apply NATCASE_morph_gen; intros; auto.
+ apply H3; trivial.
+
+ apply H1; trivial.
+
+ apply H2.
+ red in H0; specialize H0 with (1:=H4).
+ rewrite H6 in H5.
+ apply SUCCi_inv_typ in H5; auto.
+ apply val_push_var; simpl; auto.
+ rewrite <- H7.
+ clear H6 H7 x'; revert x H5.
+ apply TI_mono; auto.
+Qed.
+
+*)
+
+(*****************************************************************************)
+(** Recursor (without case analysis) *)
+
+(* NatFix O M is a fixpoint of domain Nati O with body M *)
+Definition NatFix (O M:trm) : trm.
+(*begin show*)
+left.
+exists (fun i =>
+         NATREC (fun o' f => int (V.cons f (V.cons o' i)) M) (int i O))
+       (fun j => NATFIX (Lc.Abs (tm (Lc.ilift (I.cons (tm j O) j)) M))).
+(*end show*)
+ admit.
+ admit.
+ admit.
+ admit.
+Defined.
+
+
+(** Typing rules of NatFix *)
+
+Section NatFixRules.
+
+  Variable infty : set.
+  Hypothesis infty_ord : isOrd infty.
+  Variable E : fenv.
+  Let e := tenv E.
+  Variable O U M : trm.
+  Hypothesis M_nk : ~ eq_trm M kind.
+  Hypothesis ty_O : typ e O (Ordt infty).
+  Hypothesis ty_M : typ (Prod (NatI (Ref 0)) U::OSucct O::e)
+    M (Prod (NatI (OSucc (Ref 1)))
+         (lift_rec 1 1 (subst_rec (OSucc (Ref 0)) 1 (lift_rec 1 2 U)))).
+
+  Hypothesis stab : fx_extends
+    (push_fun (push_ord E (OSucct O)) (NatI (Ref 0)) U)
+    (NatI (OSucc (Ref 1)))
+    M.
+
+  Let F i := fun o' f => int (V.cons f (V.cons o' i)) M.
+
+  Lemma morph_fix_body : forall i, morph2 (F i).
+unfold F; do 3 red; intros.
+rewrite H; rewrite H0; reflexivity.
+Qed.
+
+  Lemma ext_fun_ty : forall o i,
+    ext_fun (NATi o) (fun x => int (V.cons x (V.cons o i)) U).
+do 2 red; intros.
+rewrite H0;reflexivity.
+Qed.
+
+  Hypothesis fx_sub_U :
+    fx_sub (push_var (push_ord E (OSucct O)) (NatI (OSucc (Ref 0)))) U.
+
+  Lemma ty_fix_body : forall i j o f,
+   val_ok e i j ->
+   o < osucc (int i O) ->
+   f ∈ cc_prod (NATi o) (fun x => El(int (V.cons x (V.cons o i)) U)) ->
+   F i o f ∈
+   cc_prod (NATi (osucc o)) (fun x => El(int (V.cons x (V.cons (osucc o) i)) U)).
+unfold F; intros.
+destruct tyord_inv with (2:=ty_O) (3:=H); trivial.
+red in ty_M.
+assert (val_ok (Prod (NatI(Ref 0)) U::OSucct O::e)
+  (V.cons f (V.cons o i)) (I.cons daimon (I.cons daimon j))).
+ apply vcons_add_var; auto.
+ 3:discriminate.
+  apply vcons_add_var; auto.
+  2:discriminate.
+  split;[|apply varSAT].
+  unfold inX; simpl; rewrite El_def; trivial.
+
+  split;[|apply varSAT].
+  rewrite intProd_eq.
+  unfold inX, prod; rewrite El_def.
+  revert H1; apply eq_elim.
+  apply cc_prod_ext.
+   simpl; rewrite El_def; reflexivity.
+
+   red; intros.
+   rewrite H4; reflexivity.
+specialize ty_M with (1:=H4).
+apply in_int_not_kind in ty_M.
+2:discriminate.
+destruct ty_M as (?,_).
+rewrite intProd_eq in H5; unfold inX in H5.
+unfold prod in H5; rewrite El_def in H5.
+revert H5; apply eq_elim.
+symmetry; apply cc_prod_ext.
+ simpl; rewrite El_def.
+ reflexivity.
+
+ red; intros.
+ rewrite int_lift_rec_eq.
+ rewrite int_subst_rec_eq.
+ rewrite int_lift_rec_eq.
+ apply El_morph; apply int_morph; auto with *.
+ do 2 red.
+ intros [|[|k]].
+  compute; trivial.
+
+  unfold V.lams, V.shift; simpl.
+  reflexivity.
+
+  unfold V.lams, V.shift; simpl.
+  replace (k-0) with k; auto with *.
+Qed.
+
+  Lemma fix_body_irrel : forall i j,
+    val_ok e i j ->
+    NAT_ord_irrel (int i O) (F i) (fun o' x => El(int (V.cons x (V.cons o' i)) U)).
+Admitted.
+(*red; red; intros.
+assert (isOrd (int O i)).
+ apply ty_O in H.
+ apply isOrd_inv with infty; auto.
+red in stab.
+assert (Hstab := stab (V.cons f (V.cons o i)) (V.cons g (V.cons o' i))).
+simpl in Hstab.
+apply Hstab; clear Hstab; trivial.
+apply val_push_fun; auto.
+apply ole_lts in H1; trivial.
+apply val_push_ord; auto.
+ apply val_mono_refl; trivial.
+
+ simpl.
+ apply isOrd_plump with o'; auto.
+Qed.
+*)
+
+  Lemma fix_codom_mono : forall o o' x x' i j,
+   val_ok e i j ->
+   isOrd o' ->
+   o' ⊆ int i O ->
+   isOrd o ->
+   o ⊆ o' ->
+   x ∈ NATi o ->
+   x == x' ->
+   El (int (V.cons x (V.cons o i)) U) ⊆ El(int (V.cons x' (V.cons o' i)) U).
+Admitted.
+(*intros.
+apply fx_sub_U.
+apply val_push_var; simpl; auto.
+ apply val_push_ord; simpl; auto; change (int O (fun k => i k)) with (int O i).
+  apply val_mono_refl; trivial.
+
+  apply ole_lts; auto.
+  transitivity o'; trivial.
+
+  apply ole_lts; auto.
+
+ revert H4; apply TI_incl; auto.
+
+ rewrite <- H5.
+ revert H4; apply TI_incl; auto.
+ apply ole_lts; auto.
+Qed.
+*)
+  Hint Resolve morph_fix_body ext_fun_ty ty_fix_body fix_codom_mono fix_body_irrel.
+
+
+Let fix_typ o i j:
+  val_ok e i j ->
+  isOrd o ->
+  isOrd (int i O) ->
+  o ⊆ int i O ->
+  NATREC (F i) o
+   ∈ cc_prod (NATi o) (fun n => El (int (V.cons n (V.cons o i)) U)).
+intros.
+eapply NATREC_wt with (U:=fun o n => El(int(V.cons n (V.cons o i))U)); trivial.
+ intros.
+ apply fix_codom_mono with (1:=H); trivial.
+ transitivity o; trivial.
+
+ intros; apply ty_fix_body with (1:=H); trivial.
+ apply isOrd_plump with (int i O); auto.
+  transitivity o; trivial.
+
+  apply lt_osucc; trivial.
+
+ red; intros; apply fix_body_irrel with (1:=H); trivial.
+ transitivity o; trivial.
+Qed.
+
+
+  Lemma fix_irr i j o o' x :
+    val_ok e i j ->
+    isOrd o ->
+    isOrd o' ->
+    isOrd (int i O) ->
+    o ⊆ o' ->
+    o' ⊆ int i O ->
+    x ∈ NATi o ->
+    cc_app (NATREC (F i) o) x == cc_app (NATREC (F i) o') x.
+intros.
+apply NATREC_ord_irrel with 
+  (ord:=int i O)
+  (U:=fun o x => int (V.cons x (V.cons o i)) U); auto.
+ admit.
+ admit.
+ admit.
+Qed.
+
+
+
+Lemma fix_eqn : forall i j o n,
+  val_ok e i j ->
+  isOrd o ->
+  isOrd (int i O) ->
+  o ⊆ int i O ->
+  n ∈ NATi (osucc o) ->
+  cc_app (NATREC (F i) (osucc o)) n ==
+  cc_app (int (V.cons (NATREC (F i) o) (V.cons o i)) M) n.
+intros.
+unfold NATREC at 1.
+rewrite REC_eq; auto with *.
+apply cc_app_morph; auto with *.
+apply incl_eq.
+ red; intros.
+ rewrite sup_ax in H4; auto with *.
+ destruct H4.
+ assert (xo : isOrd x) by eauto using isOrd_inv.
+ assert (xle : x ⊆ o) by (apply olts_le; auto).
+ assert (xle' : x ⊆ int i O) by (transitivity o; trivial).
+ assert (F i x (REC (F i) x) ∈ 
+         cc_prod (NATi (osucc x)) (fun n => El (int (V.cons n (V.cons (osucc x) i)) U))).
+  apply ty_fix_body with (1:=H); trivial.
+   apply ole_lts; auto.
+
+   apply fix_typ with (1:=H); trivial.
+ assert (F i o (NATREC (F i) o) ∈ 
+         cc_prod (NATi (osucc o)) (fun n => El (int (V.cons n (V.cons (osucc o) i)) U))).
+  apply ty_fix_body with (1:=H).
+   apply ole_lts; trivial.
+
+   apply fix_typ with (1:=H); trivial.
+ rewrite cc_eta_eq with (1:=H6) in H5.
+ unfold F at 1 in H7; rewrite cc_eta_eq with (1:=H7).
+ rewrite cc_lam_def in H5|-*.
+  destruct H5.
+  destruct H8.
+  exists x0.
+   revert H5; apply TI_mono; auto with *.
+   apply osucc_mono; auto.
+  exists x1; trivial.
+  revert H8; apply eq_elim.
+  do 2 red in stab.
+  apply stab with (I.cons daimon (I.cons daimon j)) (I.cons daimon (I.cons daimon j)).
+   apply val_push_fun.
+    apply val_push_ord; trivial.
+     apply val_mono_refl; trivial.
+
+     split;[|apply varSAT].
+     unfold inX; simpl; rewrite El_def; apply ole_lts; auto.
+
+     split;[|apply varSAT].
+     unfold inX; simpl; rewrite El_def; apply ole_lts; auto.
+
+     discriminate.
+
+    split;[|apply varSAT].
+    unfold inX,prod; rewrite El_def.
+    eapply eq_elim.
+    2:eapply fix_typ with (1:=H); auto.
+    apply cc_prod_ext.
+     simpl; rewrite El_def; reflexivity.
+
+     red; intros.
+     rewrite H10; reflexivity.
+
+    split;[|apply varSAT].
+    unfold inX,prod; rewrite El_def.
+    eapply eq_elim.
+    2:eapply fix_typ with (1:=H); auto.
+    apply cc_prod_ext.
+     simpl; rewrite El_def; reflexivity.
+
+     red; intros.
+     rewrite H10; reflexivity.
+
+    red; intros.
+    apply fix_irr with (1:=H); auto with *.
+    simpl in H8; rewrite El_def in H8; trivial.
+
+   simpl; rewrite El_def; trivial.
+
+  do 2 red; intros; apply cc_app_morph; auto with *.
+  do 2 red; intros; apply cc_app_morph; auto with *.
+
+ apply sup_incl with (F:=fun o'=>F i o'(REC (F i) o')); auto with *.
+ apply lt_osucc; trivial.
+Qed.
+
+
+Lemma nat_fix_eqn : forall i j,
+  val_ok e i j ->
+  NATREC (F i) (int i O) ==
+  cc_lam (NATi (int i O))
+    (fun x => cc_app (F i (int i O) (NATREC (F i) (int i O))) x).
+intros.
+destruct tyord_inv with (2:=ty_O) (3:=H); trivial.
+apply NATREC_eqn with
+  (ord:=int i O)
+  (U:=fun o x => int (V.cons x (V.cons o i)) U); auto.
+ admit.
+ admit.
+ admit.
+Qed.
+
+
+
+Lemma equiv_piSAT_piNAT o B B' f:
+isOrd o ->
+(forall n, n ∈ NATi o -> eqSAT (Real (B n) (f n)) (B' n)) ->
+eqSAT (piSAT (mkTY (NATi o) cNAT) B f)
+      (piNATi (fun n => prodSAT (cNAT n) (B' n)) o).
+intros.
+red; intro.
+unfold piSAT, piNATi.
+apply interSAT_morph.
+split; intros.
+ destruct x as (n,xty); simpl proj1_sig.
+ simpl in xty; rewrite El_def in xty.
+ exists (exist (fun n=>_) n xty); simpl proj1_sig.
+ apply prodSAT_morph; auto.
+ rewrite Real_def; auto with *.
+ intros; apply fam_mrph; trivial.
+ revert H1; apply NATi_NAT; simpl; auto.
+
+ destruct y as (n,xty); simpl proj1_sig.
+ assert (nty : n ∈ El (mkTY (NATi o) cNAT)).
+  rewrite El_def; trivial.
+ exists (exist (fun n=>_) n nty); simpl proj1_sig.
+ apply prodSAT_morph; auto.
+ rewrite Real_def; auto with *.
+ intros; apply fam_mrph; trivial.
+ revert H1; apply NATi_NAT; simpl; auto.
+Qed.
+
+
+Lemma typ_nat_fix :
+  typ e (NatFix O M) (Prod (NatI O) (subst_rec O 1 U)).
+red; intros.
+destruct tyord_inv with (2:=ty_O)(3:=H); trivial.
+apply in_int_intro.
+2:discriminate.
+2:discriminate.
+assert (int i (NatFix O M) ∈ El(int i (Prod (NatI O) (subst_rec O 1 U)))).
+ rewrite intProd_eq.
+ eapply eq_elim.
+ 2:simpl.
+ 2:apply fix_typ with (1:=H); auto with *.
+ unfold prod; rewrite El_def; apply cc_prod_ext.
+  simpl; rewrite El_def; auto with *.
+
+  red; intros.
+  rewrite int_subst_rec_eq.
+  apply El_morph.
+  apply int_morph; auto with *.
+  intros [|[|k]]; try reflexivity.
+  exact H3.
+split; trivial.
+rewrite intProd_eq.
+rewrite Real_prod; trivial.
+ simpl tm.
+ unfold piSAT.
+ assert (inSAT (NATFIX (Lc.Abs (tm (Lc.ilift (I.cons (tm j O) j)) M)))
+   (piNATi (fun n => prodSAT (cNAT n)
+             (Real (int (V.cons n (V.cons (int i O) i)) U)
+               (cc_app (NATREC (F i) (int i O)) n))) (int i O))).
+  apply NATFIX_sat with (X:=fun o n => Real (int (V.cons n (V.cons o i)) U)
+   (cc_app (NATREC (F i) o) n)); trivial.
+   red; intros.
+   red in fx_sub_U.
+   apply fx_sub_U with (V.cons n (V.cons y i))
+      (I.cons daimon (I.cons daimon j)) (I.cons daimon (I.cons daimon j)).
+    apply val_push_var; auto with *.
+    4:discriminate.
+     apply val_push_ord; auto with *.
+     4:discriminate.
+      apply val_mono_refl; trivial.
+
+      split;[|apply varSAT].
+      unfold inX; simpl; rewrite El_def; apply ole_lts; auto.
+      transitivity y'; trivial.
+
+      split;[|apply varSAT].
+      unfold inX; simpl; rewrite El_def; apply ole_lts; auto.
+
+     rewrite realNati_def.
+     2:simpl; auto.
+     split;[|apply varSAT].
+     simpl.
+     revert H7; apply TI_incl; auto with *.
+
+     rewrite realNati_def.
+     2:simpl; auto.
+     split;[|apply varSAT].
+     simpl.
+     revert H7; apply TI_incl; auto with *.
+     apply isOrd_plump with y'; auto with *.
+     apply lt_osucc; trivial.
+
+    rewrite <- fix_irr with (1:=H) (o:=y); auto.
+    split; trivial.
+    unfold inX.
+    apply cc_prod_elim with (dom:=NATi y) (F:=fun n=>El(int(V.cons n (V.cons y i))U)); trivial.
+    apply fix_typ with (1:=H); trivial.
+    transitivity y'; trivial.
+
+   (* sat body *)
+   apply interSAT_intro.
+    exists (int i O); auto.
+    apply lt_osucc; auto.
+
+    intros.
+    destruct x as (o',?); simpl proj1_sig.
+    cbv zeta.
+    apply prodSAT_intro; intros.
+
+assert (val_ok (Prod (NatI(Ref 0)) U::OSucct O::e)
+  (V.cons (NATREC (F i) o') (V.cons o' i)) (I.cons v (I.cons (tm j O) j))).
+ apply vcons_add_var; auto.
+ 3:discriminate.
+  apply vcons_add_var; auto.
+  2:discriminate.
+  split.
+   unfold inX; simpl; rewrite El_def; trivial.
+
+   simpl int; rewrite Real_def; auto with *.
+   apply ty_O in H.
+   apply in_int_sn in H; trivial.
+
+  rewrite intProd_eq.
+  assert (NATREC (F i) o' ∈ cc_prod (NATi o')
+            (fun x => El(int(V.cons x(V.cons o' i)) U))).
+   apply fix_typ with (1:=H); trivial.
+    eauto using isOrd_inv.
+    apply olts_le in i0; trivial.
+  split.
+   unfold inX, prod; rewrite El_def.
+   revert H4; apply eq_elim; apply cc_prod_ext.
+    simpl; rewrite El_def; reflexivity.
+
+    red; intros.
+    rewrite H5; reflexivity.
+
+   rewrite Real_prod.
+   revert H3; apply equiv_piSAT_piNAT; eauto using isOrd_inv.
+   intros.
+   reflexivity.
+    
+    red; intros.
+    rewrite H6; reflexivity.
+ eapply eq_elim.
+ 2:simpl.
+ 2:apply fix_typ with (1:=H); auto with *.
+ 2:   eauto using isOrd_inv.
+ 2:   apply olts_le; trivial.
+ unfold prod; rewrite El_def; apply cc_prod_ext.
+  simpl; rewrite El_def; auto with *.
+
+  red; intros.
+  rewrite H6; reflexivity.
+
+    red in ty_M; specialize ty_M with (1:=H4).
+    apply in_int_not_kind in ty_M.
+    2:discriminate.
+    destruct ty_M.
+    replace (Lc.subst v (tm (Lc.ilift (I.cons (tm j O) j)) M))
+     with (tm (I.cons v (I.cons (tm j O) j)) M).
+     rewrite intProd_eq in H6.
+     rewrite Real_prod in H6; trivial.
+     revert H6; apply equiv_piSAT_piNAT.
+      eauto using isOrd_inv.
+     intros.
+     apply Real_morph.
+      rewrite int_lift_rec_eq.
+      rewrite int_subst_rec_eq.
+      rewrite int_lift_rec_eq.
+      apply int_morph; auto with *.
+      intros [|[|k]]; try reflexivity.
+      compute; fold minus.
+      replace (k-0) with k; auto with *.
+
+      symmetry; apply fix_eqn with (1:=H); auto.
+       eauto using isOrd_inv.
+       apply olts_le; trivial.
+
+      red; intros.
+      rewrite H8; reflexivity.
+
+    unfold Lc.subst; rewrite <- tm_substitutive.
+    apply tm_morph; auto with *.
+    intros [|[|k]].
+     unfold Lc.ilift,I.cons; simpl.
+     rewrite Lc.lift0; trivial.
+
+     unfold Lc.ilift,I.cons; simpl.
+     rewrite Lc.simpl_subst; trivial.
+     rewrite Lc.lift0; trivial.
+
+     unfold Lc.ilift,I.cons; simpl.
+     rewrite Lc.simpl_subst; trivial.
+     rewrite Lc.lift0; trivial.
+
+ revert H3; apply interSAT_morph_subset.
+  simpl; intros.
+  rewrite El_def.
+  reflexivity.
+
+  intros; simpl proj1_sig.
+  apply prodSAT_morph.
+   red; intros.
+   unfold int,NatI,iint.
+   rewrite Real_def; auto.
+   intros.
+   apply fam_mrph; auto with *.
+   revert H3; apply NATi_NAT; auto.
+
+   simpl.
+   rewrite int_subst_rec_eq.
+   apply Real_morph; [|reflexivity].
+   apply int_morph; auto with *.
+   intros [|[|k]].
+    reflexivity.
+    reflexivity.
+    reflexivity.
+
+ red; intros.
+ rewrite H4; reflexivity.
+Qed.
+
+
+Lemma nat_fix_eq : forall N,
+  typ e N (NatI O) ->
+  eq_typ e (App (NatFix O M) N)
+           (App (subst O (subst (lift 1 (NatFix O M)) M)) N).
+red; intros.
+unfold eqX.
+change
+ (app (NATREC (F i) (int i O)) (int i N) ==
+  app (int i (subst O (subst (lift 1 (NatFix O M)) M))) (int i N)).
+do 2 rewrite <- int_subst_eq.
+rewrite int_cons_lift_eq.
+rewrite nat_fix_eqn with (1:=H0); trivial.
+rewrite cc_beta_eq.
+ reflexivity.
+
+ do 2 red; intros.
+ rewrite H2; reflexivity.
+
+ red in H; specialize H with (1:=H0).
+ apply in_int_not_kind in H.
+  destruct H.
+  unfold inX in H; simpl in H; rewrite El_def in H; trivial.
+
+  discriminate.
+Qed.
+
+Lemma nat_fix_extend :
+  fx_subval E O ->
+  fx_extends E (NatI O) (NatFix O M).
+intro subO.
+do 2 red; intros.
+simpl in H0; rewrite El_def in H0.
+assert (isval := proj1 H).
+assert (isval' := proj1 (proj2 H)).
+assert (oo: isOrd (int i O)).
+ destruct tyord_inv with (2:=ty_O) (3:=isval); trivial.
+assert (oo': isOrd (int i' O)).
+ destruct tyord_inv with (2:=ty_O) (3:=isval'); trivial.
+assert (inclo: int i O ⊆ int i' O).
+ apply subO in H; trivial.
+clear subO.
+change (cc_app (NATREC (F i) (int i O)) x == cc_app (NATREC (F i') (int i' O)) x).
+revert x H0.
+elim oo using isOrd_ind; intros.
+apply TI_elim in H3; auto.
+destruct H3 as (o',?,?).
+assert (o_o' : isOrd o') by eauto using isOrd_inv.
+rewrite <- TI_mono_succ in H4; auto with *.
+rewrite <- fix_irr with (1:=isval) (o:=osucc o'); auto.
+ rewrite fix_eqn with (1:=isval); auto.
+ rewrite <- fix_irr with (1:=isval') (o:=osucc o'); auto with *.
+  rewrite fix_eqn with (1:=isval'); auto.
+  do 2 red in stab.
+  apply stab with (I.cons daimon (I.cons daimon j)) (I.cons daimon (I.cons daimon j')).
+   apply val_push_fun.
+    apply val_push_ord; auto with *.
+     split;[|apply varSAT].
+     unfold inX; simpl; rewrite El_def; apply ole_lts; auto.
+
+     split;[|apply varSAT].
+     unfold inX; simpl; rewrite El_def; apply ole_lts; auto.
+
+     discriminate.
+
+    split;[|apply varSAT].
+    unfold inX,prod; rewrite El_def.
+    eapply eq_elim.
+    2:eapply fix_typ with (1:=isval); auto.
+    apply cc_prod_ext.
+     simpl; rewrite El_def; reflexivity.
+
+     red; intros.
+     rewrite H6; reflexivity.
+
+    split;[|apply varSAT].
+    unfold inX,prod; rewrite El_def.
+    eapply eq_elim.
+    2:eapply fix_typ with (1:=isval'); auto.
+    apply cc_prod_ext.
+     simpl; rewrite El_def; reflexivity.
+
+     red; intros.
+     rewrite H6; reflexivity.
+
+    red; intros.
+    simpl in H5; rewrite El_def in H5.
+    rewrite fix_irr with (1:=isval') (o':=int i' O); auto with *.
+
+
+   simpl; rewrite El_def; trivial.
+
+  red; intros.
+  apply inclo; apply H1.
+  apply le_lt_trans with o'; trivial.
+
+ red; intros.
+ apply le_lt_trans with o'; trivial.
+Qed.
+
+Lemma nat_fix_equals :
+  fx_equals E O ->
+  fx_equals E (NatFix O M).
+red; intros.
+assert (fxs: fx_subval E O).
+ apply fx_equals_subval; trivial.
+apply nat_fix_extend in fxs.
+red in fxs.
+specialize fxs with (1:=H0).
+apply fcompat_typ_eq with (3:=fxs).
+ eapply cc_prod_is_cc_fun.
+ assert (h := typ_nat_fix _ _ (proj1 H0)).
+ apply in_int_not_kind in h.
+ 2:discriminate.
+ destruct h.
+ rewrite intProd_eq in H1.
+ unfold inX, prod in H1; rewrite El_def in H1.
+ eexact H1.
+
+ setoid_replace (int i (NatI O)) with (int i' (NatI O)).
+  eapply cc_prod_is_cc_fun.
+  assert (h := typ_nat_fix _ _ (proj1 (proj2 H0))).
+  apply in_int_not_kind in h.
+  2:discriminate.
+  destruct h.
+  rewrite intProd_eq in H1.
+  unfold inX, prod in H1; rewrite El_def in H1.
+  eexact H1.
+
+  do 2 red.
+  assert (h:= H _ _ _ _ H0).
+  apply mkTY_ext.
+   rewrite h; reflexivity.
+
+   intros; apply fam_mrph; auto.
+   revert H1; apply NATi_NAT; auto.
+   destruct tyord_inv with (2:=ty_O) (3:=proj1 H0); trivial.
+Qed.
+
+End NatFixRules.
+
+Print Assumptions typ_nat_fix.
+
+
+Lemma typ_nat_fix' : forall infty e O U M T,
+       T <> kind ->
+       isOrd infty ->
+       typ e O (Ordt infty) ->
+       typ (Prod (NatI (Ref 0)) U :: OSucct O :: e) M
+         (Prod (NatI (OSucc (Ref 1)))
+           (lift_rec 1 1 (subst_rec (OSucc (Ref 0)) 1 (lift_rec 1 2 U)))) ->
+       fx_extends (push_fun (push_ord (tinj e) (OSucct O)) (NatI (Ref 0)) U)
+         (NatI (OSucc (Ref 1))) M ->
+       fx_sub (push_var (push_ord (tinj e) (OSucct O)) (NatI (OSucc (Ref 0)))) U ->
+       sub_typ e (Prod (NatI O) (subst_rec O 1 U)) T ->
+       typ e (NatFix O M) T.
+intros.
+apply typ_subsumption with (Prod (NatI O) (subst_rec O 1 U)); auto.
+2:discriminate.
+change e with (tenv (tinj e)).
+apply typ_nat_fix with (infty:=infty); trivial.
+Qed.
+
+(****************************************************************************************)
+(** Compound judgements : typing + variance *)
+
+Definition typ_ext e M A B :=
+  fx_extends e A M /\ typ (tenv e) M (Prod A B).
+
+Definition typ_mono e M :=
+  fx_sub e M /\ typs (tenv e) M.
+
+Definition typ_monoval e M T :=
+  fx_subval e M /\ typ (tenv e) M T.
+
+Definition typ_impl e M T :=
+  fx_equals e M /\ typ (tenv e) M T.
+
+Instance typ_impl_morph e : Proper (eq_trm ==> eq_trm ==> iff) (typ_impl e).
+apply morph_impl_iff2; auto with *.
+do 4 red; intros.
+destruct H1; split.
+ red; intros.
+ rewrite <- H; eauto.
+
+ rewrite <- H; rewrite <- H0; eauto.
+Qed.
+
+Lemma typ_var_impl : forall e n t T,
+    spec_var e n = false ->
+    nth_error (tenv e) n = value t ->
+    t <> kind ->
+    T <> kind ->
+    sub_typ (tenv e) (lift (S n) t) T ->
+    typ_impl e (Ref n) T.
+intros.
+split.
+ apply fx_eq_noc; apply noc_var; trivial.
+
+ apply typ_subsumption with (lift (S n) t); trivial.
+  apply typ_var; trivial.
+
+  destruct t as [(t,tm)|]; simpl in *; auto.
+  discriminate.
+Qed.
+
+  Lemma impl_abs : forall e s1 U T T' M,
+    T <> kind ->
+    U <> kind ->
+    s1=prop \/ s1=kind ->
+    eq_typ (tenv e) T T' ->
+    typ_impl e T s1 ->
+    typ_impl (push_var e T) M U ->
+    typ_impl e (Abs T M) (Prod T' U).
+intros.
+destruct H3; destruct H4.
+split.
+ apply fx_eq_abs; trivial.
+
+ apply typ_conv with (Prod T U); auto.
+  apply typ_abs; trivial.
+  destruct H1; subst s1; red; auto.
+
+  apply eq_typ_prod; trivial.
+  reflexivity.
+
+  discriminate.
+
+  discriminate.
+Qed.
+
+Lemma impl_app : forall e u v V Ur T,
+  T <> kind ->
+  V <> kind ->
+  Ur <> kind ->
+  sub_typ (tenv e) (subst v Ur) T ->
+  typ_impl e u (Prod V Ur) ->
+  typ_impl e v V ->
+  typ_impl e (App u v) T.
+intros.
+destruct H3.
+destruct H4.
+split.
+ apply fx_eq_app; trivial.
+
+ apply typ_subsumption with (subst v Ur); trivial.
+  apply typ_app with V; auto.
+
+  destruct Ur as [(Ur,Urm)|]; simpl; trivial.
+  discriminate.
+Qed.
+
+  Lemma NATi_fx_sub : forall e o O,
+    isOrd o ->
+    typ_monoval e O (Ordt o) ->
+    fx_sub e (NatI O).
+destruct 2.
+apply NATi_sub with (o:=o); trivial.
+Qed.
+
+  Lemma OSucc_fx_sub : forall e O o,
+    isOrd o ->
+    typ_monoval e O (Ordt o)->
+    typ_monoval e (OSucc O) (Ordt (osucc o)).
+destruct 2.
+split.
+ apply OSucc_sub; trivial.
+
+ red; simpl; intros.
+ apply in_int_intro; try discriminate.
+ assert (osucc (int i O) ∈ El (int i (Ordt (osucc o)))).
+  simpl; rewrite El_def.
+  apply lt_osucc_compat; trivial.
+  destruct tyord_inv with (2:=H1)(3:=H2); trivial.
+ split; trivial.
+ unfold int at 1, Ordt, cst, iint.
+ rewrite Real_def; auto with *.
+  assert (h:= H1 _ _ H2).
+  apply in_int_sn in h.
+  simpl; trivial.
+
+  simpl.
+  apply lt_osucc_compat; trivial.
+  destruct tyord_inv with (2:=H1)(3:=H2); trivial.
+Qed.
+
+  Lemma typ_var_mono : forall e n t T,
+    ords e n = true ->
+    nth_error (tenv e) n = value t ->
+    T <> kind ->
+    t <> kind ->
+    sub_typ (tenv e) (lift (S n) t) T ->
+    typ_monoval e (Ref n) T.
+intros.
+split.
+ apply var_sub; trivial.
+
+ apply typ_subsumption with (lift (S n) t); trivial.
+  apply typ_var; trivial.
+
+  destruct t as [(t,tm)|]; simpl in *; auto.
+  discriminate.
+Qed.
+
+  Lemma ext_abs : forall e U T M,
+    T <> kind ->
+    U <> kind ->
+    typ_mono e T ->
+    typ_impl (push_var e T) M U ->
+    typ_ext e (Abs T M) T U.
+intros.
+destruct H1; destruct H2; split.
+ apply fx_abs with U; trivial.
+
+ apply typ_abs; trivial.
+Qed.
+
+(*************)
+(*
+Lemma impl_natcase : forall o e O P fZ fS n T,
+       isOrd o ->
+       typ_mono e O (Ordt o) ->
+       sub_typ (tenv e) (App P n) T -> 
+       typ_impl e fZ (App P Zero) ->
+       typ_impl (push_var e (NatI O)) fS
+         (App (lift 1 P) (App (Succ (lift 1 O)) (Ref 0))) ->
+       typ_impl e n (NatI (OSucc O)) ->
+       typ_impl e (Natcase fZ fS n) T.
+intros.
+destruct H0.
+destruct H2.
+destruct H3.
+simpl in H7.
+destruct H4.
+split.
+ apply Natcase_fx_eq with o O; trivial.
+
+ apply typ_natcase' with o O P; trivial.
+Qed.
+*)
+
+  Lemma impl_call : forall e n x t u T,
+    ords e n = false ->
+    fixs e n = Some t ->
+    T <> kind ->
+    t <> kind ->
+    u <> kind ->
+    nth_error (tenv e) n = value (Prod t u) ->
+    sub_typ (tenv e) (subst x (lift_rec (S n) 1 u)) T ->
+    typ_impl e x (lift (S n) t) ->
+    typ_impl e (App (Ref n) x) T.
+intros.
+destruct H6.
+assert (typ (tenv e) (Ref n) (Prod (lift (S n) t) (lift_rec (S n) 1 u))).
+ apply typ_var0; rewrite H4; split;[discriminate|].
+ apply sub_refl.
+admit.
+(* unfold lift; rewrite eq_lift_prod.
+ reflexivity.*)
+split.
+ apply fx_eq_rec_call with t (lift_rec (S n) 1 u); trivial.
+
+ apply typ_subsumption with (subst x (lift_rec (S n) 1 u)); auto.
+ 2:destruct u as [(u,um)|]; trivial.
+ 2:discriminate.
+ apply typ_app with (lift (S n) t); trivial.
+ destruct t as [(t,tm)|]; trivial.
+ discriminate.
+ destruct u as [(u,um)|]; trivial.
+ discriminate.
+Qed.
+
+
+Lemma typ_nat_fix'' : forall infty e O U M T,
+       isOrd infty ->
+       T <> kind ->
+       sub_typ (tenv e) (Prod (NatI O) (subst_rec O 1 U)) T ->
+       typ (tenv e) O (Ordt infty) ->
+       typ_mono (push_var (push_ord e (OSucct O)) (NatI (OSucc (Ref 0)))) U ->
+       typ_ext (push_fun (push_ord e (OSucct O)) (NatI (Ref 0)) U)
+         M (NatI (OSucc (Ref 1)))
+           (lift_rec 1 1 (subst_rec (OSucc (Ref 0)) 1 (lift_rec 1 2 U))) ->
+       typ (tenv e) (NatFix O M) T.
+intros.
+destruct H3; destruct H4.
+apply typ_subsumption with (2:=H1); trivial.
+2:discriminate.
+apply typ_nat_fix with infty; trivial.
+Qed.
+
+  Lemma typ_ext_fix : forall eps e O U M,
+    isOrd eps ->
+    typ_monoval e O (Ordt eps) ->
+    typ_ext (push_fun (push_ord e (OSucct O)) (NatI (Ref 0)) U) M
+      (NatI (OSucc (Ref 1))) (lift_rec 1 1 (subst_rec (OSucc (Ref 0)) 1 (lift_rec 1 2 U))) ->
+    fx_sub (push_var (push_ord e (OSucct O)) (NatI (OSucc (Ref 0)))) U ->
+    typ_ext e (NatFix O M) (NatI O) (subst_rec O 1 U).
+intros eps e O U M eps_ord tyO tyM tyU.
+destruct tyO as (inclO,tyO).
+destruct tyM as (extM,tyM).
+assert (tyF: typ (tenv e) (NatFix O M) (Prod (NatI O) (subst_rec O 1 U))).
+ apply typ_nat_fix with eps; trivial.
+split; trivial.
+apply nat_fix_extend with eps U; trivial.
+Qed.
+
+  Lemma typ_impl_fix : forall eps e O U M,
+    isOrd eps ->
+    typ_impl e O (Ordt eps) ->
+    typ_ext (push_fun (push_ord e (OSucct O)) (NatI (Ref 0)) U) M
+      (NatI (OSucc (Ref 1))) (lift_rec 1 1 (subst_rec (OSucc (Ref 0)) 1 (lift_rec 1 2 U))) ->
+    fx_sub (push_var (push_ord e (OSucct O)) (NatI (OSucc (Ref 0)))) U ->
+    typ_impl e (NatFix O M) (Prod (NatI O) (subst_rec O 1 U)).
+intros eps e O U M eps_ord tyO tyM tyU.
+destruct tyO as (inclO,tyO).
+destruct tyM as (extM,tyM).
+assert (tyF: typ (tenv e) (NatFix O M) (Prod (NatI O) (subst_rec O 1 U))).
+ apply typ_nat_fix with eps; trivial.
+split; trivial.
+apply nat_fix_equals with eps U; trivial.
+Qed.
+
+
+(************************************************************************)
+(** Two examples of derived principles:
+    - the standard recursor for Nat
+    - subtraction with size information
+*)
+(*
+Section Example.
+
+Definition nat_ind_typ :=
+   Prod (Prod (NatI (Ord omega)) prop) (* P : nat -> Prop *)
+  (Prod (App (Ref 0) Zero)
+  (Prod (Prod (NatI (Ord omega)) (Prod (App (Ref 2) (Ref 0))
+                        (App (Ref 3) (App (Succ (Ord omega)) (Ref 1)))))
+  (Prod (NatI (Ord omega)) (App (Ref 3) (Ref 0))))).
+
+Definition nat_ind :=
+   Abs (*P*)(Prod (NatI (Ord omega)) prop) (* P : nat -> Prop *)
+  (Abs (*fZ*) (App (Ref 0) Zero)
+  (Abs (*fS*) (Prod (*n*)(NatI (Ord omega)) (Prod (App (Ref 2) (Ref 0))
+                                   (App (Ref 3) (App (Succ (Ord omega)) (Ref 1)))))
+  (NatFix (Ord omega)
+    (*o,Hrec*)
+    (Abs (*n*)(NatI (OSucc (Ref 1)))
+      (Natcase
+        (Ref 4)
+        (*k*)(App (App (Ref 4) (Ref 0))
+                  (App (Ref 2) (Ref 0)))
+        (Ref 0)))))).
+
+
+
+Lemma nat_ind_def :
+  forall e, typ e nat_ind nat_ind_typ.
+assert (eq_term Nat (NatI (Ord omega))).
+ red; simpl.
+ red; unfold NAT; reflexivity.
+unfold nat_ind, nat_ind_typ; intros.
+apply typ_abs; try discriminate.
+apply typ_abs; try discriminate.
+apply typ_abs; try discriminate.
+
+set (E0 := Prod (NatI (Ord omega))
+                 (Prod (App (Ref 2) (Ref 0))
+                    (App (Ref 3) (App (SuccI (Ord omega)) (Ref 1))))
+               :: App (Ref 0) Zero :: Prod (NatI (Ord omega)) prop :: e) in |-*.
+change E0 with (tenv (tinj E0)).
+apply typ_nat_fix'' with (osucc omega) (App (Ref 4) (Ref 0)); auto.
+ (* sub *)
+ apply sub_refl.
+ apply eq_typ_prod.
+  reflexivity.
+
+  eapply eq_typ_morph;[reflexivity| |reflexivity].
+  simpl; do 2 red; simpl; intros.
+  unfold V.lams, V.shift; simpl.
+  apply cc_app_morph; apply H0.
+
+ (* ord *)
+ red; simpl; intros.
+ apply lt_osucc; trivial.
+
+ (* codom mono *)
+ split.
+  apply fx_equals_sub.
+  apply fx_eq_noc.
+  apply noc_app.
+   apply noc_var; reflexivity.
+   apply noc_var; reflexivity.
+
+  red; intros; simpl; exact I.
+
+ (* fix body *)
+ apply ext_abs; try discriminate.
+  apply NATi_fx_sub with (o:=osucc (osucc omega)); auto.
+  apply OSucc_fx_sub; auto.
+  apply typ_var_mono with (OSucct (Ord omega)); auto; try discriminate.
+  red; simpl; intros; trivial.
+
+  apply impl_natcase with (osucc omega) (Ref 2) (Ref 5); auto.
+   eapply typ_var_mono.
+    compute; reflexivity.
+    simpl; reflexivity.
+    discriminate.
+
+    simpl tenv; apply sub_refl.
+    red; simpl; intros; reflexivity.
+
+   simpl tenv.
+   apply sub_refl.
+   red; simpl; intros.
+   unfold V.lams, V.shift; simpl.
+   reflexivity.
+
+   (* branch 0 *)
+   eapply typ_var_impl.
+    compute; reflexivity.
+    simpl nth_error.
+    reflexivity.
+    discriminate.
+
+    apply sub_refl; red; simpl; intros.
+    unfold V.lams, V.shift; simpl.
+    reflexivity.
+
+   (* branch S *)
+   apply impl_app with (App (Ref 6) (Ref 0))
+     (App (Ref 7) (App (SuccI (Ref 4)) (Ref 1))); try discriminate.
+    simpl tenv.
+    apply sub_refl; red; intros; simpl.
+    unfold V.lams, V.shift; simpl.
+    reflexivity.
+
+    apply impl_app with (NatI (Ord omega))
+      (Prod (App (Ref 7) (Ref 0)) (App (Ref 8) (App (SuccI (Ord omega)) (Ref 1))));
+      try discriminate.
+     simpl tenv.
+     unfold subst; rewrite eq_subst_prod.
+     apply sub_typ_covariant.
+      red; simpl; intros; reflexivity.
+
+     apply sub_refl.
+     red; intros; simpl.
+     apply cc_app_morph; [reflexivity|].
+     assert (i 1 ∈ NATi (i 4)).
+      generalize (H0 1 _ (eq_refl _)); simpl.
+      unfold V.lams, V.shift; simpl.
+      trivial.
+     rewrite beta_eq.
+      rewrite beta_eq; auto with *.
+       reflexivity.
+       red; intros; apply inr_morph; trivial.
+
+      red; intros; apply inr_morph; trivial.
+
+      apply NATi_NAT in H1; trivial.
+      generalize (H0 4 _ (eq_refl _)); simpl; intro.
+      apply isOrd_inv with (osucc omega); auto.
+
+     eapply typ_var_impl.
+      compute; reflexivity.
+      simpl; reflexivity.
+      discriminate.
+
+      apply sub_refl.
+      red; intros; simpl.
+      unfold V.lams, V.shift; simpl.
+      reflexivity.
+
+     eapply typ_var_impl.
+      compute; reflexivity.
+      simpl; reflexivity.
+      discriminate.
+
+      red; intros; simpl.
+      simpl in H1.
+      unfold V.lams, V.shift in H1; simpl in H1.
+      apply NATi_NAT in H1; trivial.
+      generalize (H0 3 _ (eq_refl _)); simpl; intro.
+      apply isOrd_inv with (osucc omega); auto.
+
+    eapply impl_call.
+     compute; trivial.
+     simpl; reflexivity.
+     discriminate.
+     2:simpl; reflexivity.
+     discriminate.
+
+     apply sub_refl; red; intros; simpl.
+     unfold V.lams, V.shift; simpl.
+     reflexivity.
+
+     eapply typ_var_impl.
+      compute; reflexivity.
+      simpl; reflexivity.
+      discriminate.
+
+      apply sub_refl; red; intros; simpl.
+      reflexivity.
+
+   (* Scrutinee *)
+   eapply typ_var_impl.
+    compute; reflexivity.
+    simpl; reflexivity.
+    discriminate.
+
+    apply sub_refl; red; intros; simpl.
+    reflexivity.
+Qed.
+
+
+(* Subtraction *)
+
+Definition minus O :=
+  NatFix O
+    (*o,Hrec*)
+    (Abs (*n*) (NatI (OSucc (Ref 1)))
+    (Abs (*m*) (NatI (Ord omega))
+    (Natcase
+       Zero
+       (*n'*)
+       (Natcase
+         (Ref 2)
+         (*m'*)
+         (App (App (Ref 4) (Ref 1)) (Ref 0))
+         (Ref 1))
+       (Ref 1)))).
+
+Definition minus_typ O := Prod (NatI O) (Prod (NatI (Ord omega)) (NatI (lift 2 O))).
+
+
+
+Lemma minus_def :
+  forall e infty O,
+  isOrd infty ->
+  typ e O (Ord infty) ->
+  typ e (minus O) (minus_typ O).
+intros.
+unfold minus, minus_typ.
+change e with (tenv (tinj e)).
+apply typ_nat_fix'' with infty (Prod (NatI (Ord omega)) (NatI (Ref 2))); auto.
+ (* sub *)
+ apply sub_refl.
+ apply eq_typ_prod.
+  reflexivity.
+
+  rewrite eq_subst_prod.
+  apply eq_typ_prod.
+   red; intros; simpl; reflexivity.
+
+   red; intros; simpl.
+   unfold lift; rewrite int_lift_rec_eq.
+   rewrite V.lams0.
+   unfold V.lams, V.shift; simpl; reflexivity.
+
+ (* codom mono *)
+ split;[|red; intros; simpl; exact I].
+ apply fx_sub_prod.
+  apply fx_eq_noc.
+  red; simpl; reflexivity.
+
+  apply NATi_sub with infty; trivial.
+  simpl.
+  apply typ_var0; split; [discriminate|].
+  red; intros; simpl.
+  unfold lift in H2; rewrite int_lift_rec_eq in H2.
+  rewrite V.lams0 in H2.
+  simpl in H2.
+  apply le_lt_trans with (2:=H2); trivial.
+  apply H0.
+  red; intros.
+  generalize (H1 (3+n) _ H3).
+  destruct T as [(T,Tm)|]; simpl; trivial.
+
+  apply var_sub.
+  compute; reflexivity.
+
+ (* fix body *)
+ apply ext_abs; try discriminate.
+  apply NATi_fx_sub with (o:=osucc infty); auto.
+  apply OSucc_fx_sub; auto.
+  eapply typ_var_mono.
+   compute; reflexivity.
+   simpl; reflexivity.
+   discriminate.
+  red; simpl; intros; trivial.
+  apply weakening0 in H0; apply weakeningS with (A:=OSucct O) in H0.
+  apply weakeningS with (A:=Prod(NatI(Ref 0))(Prod(NatI(Ord omega))(NatI(Ref 2)))) in H0.
+  apply H0 in H1.
+  simpl in H1.
+  unfold lift in H1; rewrite int_lift_rec_eq in H1.
+  apply le_lt_trans with (3:=H1); trivial.
+
+ rewrite eq_lift_prod.
+ rewrite eq_subst_prod.
+ unfold lift1; rewrite eq_lift_prod.
+ apply impl_abs.
+  discriminate.
+
+  red; intros; simpl.
+  reflexivity.
+
+  red; intros; simpl; auto with *.
+
+ match goal with |- typ_impl ?e _ _ => set (E:=e) end.
+ assert (typ_impl E (Ref 1) (NatI (OSucc (Ref 3)))).
+  eapply typ_var_impl.
+   compute; reflexivity.
+   simpl; reflexivity.
+   discriminate.
+  apply sub_refl.
+  red; intros; simpl; reflexivity.
+ apply impl_natcase with infty (Ref 3)
+    (Abs (NatI (OSucc (Ref 3))) (NatI (OSucc (Ref 4)))); auto.
+  Focus 2.
+  apply sub_refl.
+  rewrite eq_typ_betar.
+  3:discriminate.
+   red; intros; simpl.
+   unfold V.lams, V.shift; simpl.
+   reflexivity.
+
+   apply H1.
+
+  (* ord *)
+  eapply typ_var_mono.
+   compute;reflexivity.
+   simpl; reflexivity.
+   discriminate.
+  red; intros; simpl.
+  unfold lift in H3; rewrite int_lift_rec_eq in H3.
+  rewrite V.lams0 in H3.
+  simpl in H3.
+  apply le_lt_trans with (2:=H3); trivial.
+  apply H0.
+  red; intros.
+  generalize (H2 (4+n) _ H4).
+  destruct T as [(T,Tm)|]; simpl; auto.
+
+  (* branch 0 *)
+  split.
+   red; intros; simpl; reflexivity.
+  assert (tyz : typ (tenv E) Zero (NatI (OSucc (Ref 3)))).
+    apply typ_Zero with infty; trivial.
+    apply typ_var0; split; [discriminate|].
+    red; intros; simpl.
+    unfold lift in H3; rewrite int_lift_rec_eq in H3.
+    rewrite V.lams0 in H3.
+    simpl in H3.
+    apply le_lt_trans with (2:=H3); trivial.
+    apply H0.
+    red; intros.
+    generalize (H2 (4+n) _ H4).
+    destruct T as [(T,Tm)|]; simpl; trivial.
+  apply typ_conv with (NatI (OSucc (Ref 3))); trivial.
+  2:discriminate.
+  rewrite eq_typ_betar; trivial.
+  2:discriminate.
+  red; intros; simpl.
+  reflexivity.
+
+  (* branch S *)
+  assert (typ_impl (push_var E (NatI (Ref 3))) (Ref 1) (NatI (Ord (osucc omega)))).
+   eapply typ_var_impl.
+    compute; reflexivity.
+    simpl; reflexivity.
+    discriminate.
+   apply sub_refl.
+   red; intros; simpl.
+   unfold NATi at 2; rewrite TI_mono_succ; auto.
+   apply NAT_eq.
+  apply impl_natcase with (osucc omega) (Ord omega)
+     (Abs (NatI (OSucct (Ord omega))) (NatI (OSucc (Ref 5)))); auto.
+   Focus 2.
+   apply sub_refl.
+   rewrite eq_typ_betar.
+   3:discriminate.
+    unfold lift; rewrite eq_lift_abs.
+    rewrite eq_typ_betar.
+    3:discriminate.
+     red; intros; simpl; reflexivity.
+     apply typ_conv with (NatI (OSucc (lift_rec 1 0 (Ref 3)))).
+     3:discriminate.
+      apply typ_SuccI with (o:=infty); trivial.
+      apply typ_var0; split;[discriminate|].
+      red; intros; simpl.
+      unfold lift in H4; rewrite int_lift_rec_eq in H4.
+      rewrite V.lams0 in H4.
+      simpl in H4.
+      apply le_lt_trans with (2:=H4); trivial.
+      apply H0.
+      red; intros.
+      generalize (H3 (5+n) _ H5).
+      destruct T as [(T,Tm)|]; simpl; trivial.
+
+      apply typ_var0; split;[discriminate|].
+      apply sub_refl; red; intros; simpl.
+      reflexivity.
+
+     red; intros; simpl.
+     reflexivity.
+
+     apply H2.
+
+   (* ord *)
+   split.
+    red; intros; simpl; reflexivity.
+
+    red; intros; simpl.
+    apply lt_osucc; trivial.
+
+  (* branch 0 *)
+  eapply typ_var_impl.
+   compute; reflexivity.
+   simpl; reflexivity.
+   discriminate.
+  apply sub_refl.
+  rewrite eq_typ_betar.
+  3:discriminate.
+   red; intros; simpl.
+   unfold V.lams, V.shift; simpl; reflexivity.
+
+   eapply typ_Zero with (osucc omega); auto.
+   red; intros; simpl.
+   apply lt_osucc; trivial.
+
+  (* branch S *)    
+  apply impl_app with (NatI (Ord omega)) (NatI (OSucc (Ref 6))).
+   discriminate.
+   discriminate.
+
+   unfold lift; rewrite eq_lift_abs.
+   apply sub_refl.
+   rewrite eq_typ_betar.
+   3:discriminate.
+    red; intros; simpl.
+    unfold V.lams, V.shift; simpl.
+    reflexivity.
+
+    apply typ_conv with (NatI (OSucc (lift_rec 1 0 (Ord omega)))).
+    3:discriminate.
+     apply typ_SuccI with (o:=osucc omega); auto.
+      red; intros; simpl.
+      apply lt_osucc; trivial.
+
+      apply typ_var0; split;[discriminate|].
+      apply sub_refl; red; intros; simpl.
+      reflexivity.
+
+     red; intros; simpl.
+     reflexivity.
+
+   eapply impl_call.
+    compute; reflexivity.
+    simpl; reflexivity.
+    discriminate.
+    2:simpl; reflexivity.
+    discriminate.
+
+    unfold subst, lift1; rewrite eq_lift_prod.
+    rewrite eq_subst_prod.
+    apply sub_typ_covariant.
+     red; intros; simpl; reflexivity.
+
+     red; intros; simpl.
+     rewrite int_subst_rec_eq in H4.
+     simpl in H4; unfold V.lams, V.shift in H4; simpl in H4.
+     assert (isOrd (i 6)).
+      generalize (H3 6 _ (reflexivity _)).
+      simpl; intro.
+      rewrite V.lams0 in H5.
+      apply isOrd_inv with (2:=H5).      
+      apply isOrd_succ.
+      assert (val_ok e (V.shift 7 i)).
+       red; intros.
+       generalize (H3 (7+n) _ H6).
+       destruct T as [(T,Tm)|]; simpl; auto.
+      apply H0 in H6.
+      simpl in H6.
+      apply isOrd_inv with infty; trivial.
+     revert H4; apply TI_incl; auto.
+
+    eapply typ_var_impl.
+     compute; reflexivity.
+     simpl; reflexivity.
+     discriminate.
+
+     apply sub_refl.
+     red; intros; simpl.
+     reflexivity.
+
+     eapply typ_var_impl.
+      compute; reflexivity.
+      simpl; reflexivity.
+      discriminate.
+
+      apply sub_refl.
+      red; intros; simpl.
+      reflexivity.
+Qed.
+
+End Example.
+
+Print Assumptions minus_def.
+*)
